src/parser: Cleaner name resolution
Now, scopes are handled more intuitively, very much like OCaml:
local opens really shadow previous local definitions, etc.

The elaborator now relies on a cleaner implementation for name
resolution in src/parser/env.fs, based on keeping one single list
with all declarations interleaved, instead of keeping separate
lists for local definitions, recursive definitions, open
namespaces and module abbrevs.

Thus, this commit also fixes some spurious shadowings, which were
missed in some examples.

This commit heavily relies on the fact that, whenever a name of
the form Namespace.ident shows up, Namespace is always the name of
a valid module (not an effect or a data constructor). So, now,
Namespace is first separately resolved as a module, then the
definition is looked up into the given module.

This commit currently allows module name resolution at
open, let open, and module abbrevs, but I claim that this can be
easily changed and reverted to the previous behavior of requiring
fully qualified module names.

src/ocaml-output/FStar_Parser_Env.ml
@@ -1,8 +1,153 @@
 
 open Prims
 
+type local_binding =
+(FStar_Ident.ident * FStar_Syntax_Syntax.bv * Prims.bool)
+
+
+type rec_binding =
+(FStar_Ident.ident * FStar_Ident.lid * FStar_Syntax_Syntax.delta_depth)
+
+
+type module_abbrev =
+(FStar_Ident.ident * FStar_Ident.lident)
+
+
+type open_kind =
+| Open_module
+| Open_namespace
+
+
+let is_Open_module = (fun _discr_ -> (match (_discr_) with
+| Open_module (_) -> begin
+true
+end
+| _ -> begin
+false
+end))
+
+
+let is_Open_namespace = (fun _discr_ -> (match (_discr_) with
+| Open_namespace (_) -> begin
+true
+end
+| _ -> begin
+false
+end))
+
+
+type open_module_or_namespace =
+(FStar_Ident.lident * open_kind)
+
+
+type record_or_dc =
+{typename : FStar_Ident.lident; constrname : FStar_Ident.lident; parms : FStar_Syntax_Syntax.binders; fields : (FStar_Syntax_Syntax.fieldname * FStar_Syntax_Syntax.typ) Prims.list; is_record : Prims.bool}
+
+
+let is_Mkrecord_or_dc : record_or_dc  ->  Prims.bool = (Obj.magic ((fun _ -> (FStar_All.failwith "Not yet implemented:is_Mkrecord_or_dc"))))
+
+
+type scope_mod =
+| Local_binding of local_binding
+| Rec_binding of rec_binding
+| Module_abbrev of module_abbrev
+| Open_module_or_namespace of open_module_or_namespace
+| Top_level_def of FStar_Ident.ident
+| Record_or_dc of record_or_dc
+
+
+let is_Local_binding = (fun _discr_ -> (match (_discr_) with
+| Local_binding (_) -> begin
+true
+end
+| _ -> begin
+false
+end))
+
+
+let is_Rec_binding = (fun _discr_ -> (match (_discr_) with
+| Rec_binding (_) -> begin
+true
+end
+| _ -> begin
+false
+end))
+
+
+let is_Module_abbrev = (fun _discr_ -> (match (_discr_) with
+| Module_abbrev (_) -> begin
+true
+end
+| _ -> begin
+false
+end))
+
+
+let is_Open_module_or_namespace = (fun _discr_ -> (match (_discr_) with
+| Open_module_or_namespace (_) -> begin
+true
+end
+| _ -> begin
+false
+end))
+
+
+let is_Top_level_def = (fun _discr_ -> (match (_discr_) with
+| Top_level_def (_) -> begin
+true
+end
+| _ -> begin
+false
+end))
+
+
+let is_Record_or_dc = (fun _discr_ -> (match (_discr_) with
+| Record_or_dc (_) -> begin
+true
+end
+| _ -> begin
+false
+end))
+
+
+let ___Local_binding____0 = (fun projectee -> (match (projectee) with
+| Local_binding (_63_34) -> begin
+_63_34
+end))
+
+
+let ___Rec_binding____0 = (fun projectee -> (match (projectee) with
+| Rec_binding (_63_37) -> begin
+_63_37
+end))
+
+
+let ___Module_abbrev____0 = (fun projectee -> (match (projectee) with
+| Module_abbrev (_63_40) -> begin
+_63_40
+end))
+
+
+let ___Open_module_or_namespace____0 = (fun projectee -> (match (projectee) with
+| Open_module_or_namespace (_63_43) -> begin
+_63_43
+end))
+
+
+let ___Top_level_def____0 = (fun projectee -> (match (projectee) with
+| Top_level_def (_63_46) -> begin
+_63_46
+end))
+
+
+let ___Record_or_dc____0 = (fun projectee -> (match (projectee) with
+| Record_or_dc (_63_49) -> begin
+_63_49
+end))
+
+
 type env =
-{curmodule : FStar_Ident.lident Prims.option; curmonad : FStar_Ident.ident Prims.option; modules : (FStar_Ident.lident * FStar_Syntax_Syntax.modul) Prims.list; open_namespaces : FStar_Ident.lident Prims.list; modul_abbrevs : (FStar_Ident.ident * FStar_Ident.lident) Prims.list; sigaccum : FStar_Syntax_Syntax.sigelts; localbindings : (FStar_Ident.ident * FStar_Syntax_Syntax.bv * Prims.bool) Prims.list; recbindings : (FStar_Ident.ident * FStar_Ident.lid * FStar_Syntax_Syntax.delta_depth) Prims.list; sigmap : (FStar_Syntax_Syntax.sigelt * Prims.bool) FStar_Util.smap; default_result_effect : FStar_Ident.lident; iface : Prims.bool; admitted_iface : Prims.bool; expect_typ : Prims.bool}
+{curmodule : FStar_Ident.lident Prims.option; curmonad : FStar_Ident.ident Prims.option; modules : (FStar_Ident.lident * FStar_Syntax_Syntax.modul) Prims.list; scope_mods : scope_mod Prims.list; sigaccum : FStar_Syntax_Syntax.sigelts; sigmap : (FStar_Syntax_Syntax.sigelt * Prims.bool) FStar_Util.smap; default_result_effect : FStar_Ident.lident; iface : Prims.bool; admitted_iface : Prims.bool; expect_typ : Prims.bool}
 
 
 let is_Mkenv : env  ->  Prims.bool = (Obj.magic ((fun _ -> (FStar_All.failwith "Not yet implemented:is_Mkenv"))))
@@ -32,22 +177,15 @@ end))
 
 
 let ___Term_name____0 = (fun projectee -> (match (projectee) with
-| Term_name (_63_30) -> begin
-_63_30
+| Term_name (_63_63) -> begin
+_63_63
 end))
 
 
 let ___Eff_name____0 = (fun projectee -> (match (projectee) with
-| Eff_name (_63_33) -> begin
-_63_33
+| Eff_name (_63_66) -> begin
+_63_66
 end))
-
-
-type record_or_dc =
-{typename : FStar_Ident.lident; constrname : FStar_Ident.lident; parms : FStar_Syntax_Syntax.binders; fields : (FStar_Syntax_Syntax.fieldname * FStar_Syntax_Syntax.typ) Prims.list; is_record : Prims.bool}
-
-
-let is_Mkrecord_or_dc : record_or_dc  ->  Prims.bool = (Obj.magic ((fun _ -> (FStar_All.failwith "Not yet implemented:is_Mkrecord_or_dc"))))
 
 
 let open_modules : env  ->  (FStar_Ident.lident * FStar_Syntax_Syntax.modul) Prims.list = (fun e -> e.modules)
@@ -67,49 +205,49 @@ let qual : FStar_Ident.lident  ->  FStar_Ident.ident  ->  FStar_Ident.lident = F
 
 let qualify : env  ->  FStar_Ident.ident  ->  FStar_Ident.lident = (fun env id -> (match (env.curmonad) with
 | None -> begin
-(let _158_95 = (current_module env)
-in (qual _158_95 id))
+(let _158_172 = (current_module env)
+in (qual _158_172 id))
 end
 | Some (monad) -> begin
-(let _158_97 = (let _158_96 = (current_module env)
-in (qual _158_96 monad))
-in (FStar_Syntax_Util.mk_field_projector_name_from_ident _158_97 id))
+(let _158_174 = (let _158_173 = (current_module env)
+in (qual _158_173 monad))
+in (FStar_Syntax_Util.mk_field_projector_name_from_ident _158_174 id))
 end))
 
 
-let new_sigmap = (fun _63_52 -> (match (()) with
+let new_sigmap = (fun _63_79 -> (match (()) with
 | () -> begin
 (FStar_Util.smap_create (Prims.parse_int "100"))
 end))
 
 
-let empty_env : Prims.unit  ->  env = (fun _63_53 -> (match (()) with
+let empty_env : Prims.unit  ->  env = (fun _63_80 -> (match (()) with
 | () -> begin
-(let _158_101 = (new_sigmap ())
-in {curmodule = None; curmonad = None; modules = []; open_namespaces = []; modul_abbrevs = []; sigaccum = []; localbindings = []; recbindings = []; sigmap = _158_101; default_result_effect = FStar_Syntax_Const.effect_Tot_lid; iface = false; admitted_iface = false; expect_typ = false})
+(let _158_178 = (new_sigmap ())
+in {curmodule = None; curmonad = None; modules = []; scope_mods = []; sigaccum = []; sigmap = _158_178; default_result_effect = FStar_Syntax_Const.effect_Tot_lid; iface = false; admitted_iface = false; expect_typ = false})
 end))
 
 
 let sigmap : env  ->  (FStar_Syntax_Syntax.sigelt * Prims.bool) FStar_Util.smap = (fun env -> env.sigmap)
 
 
-let has_all_in_scope : env  ->  Prims.bool = (fun env -> (FStar_List.existsb (fun _63_59 -> (match (_63_59) with
-| (m, _63_58) -> begin
+let has_all_in_scope : env  ->  Prims.bool = (fun env -> (FStar_List.existsb (fun _63_86 -> (match (_63_86) with
+| (m, _63_85) -> begin
 (FStar_Ident.lid_equals m FStar_Syntax_Const.all_lid)
 end)) env.modules))
 
 
 let default_total : env  ->  env = (fun env -> (
 
-let _63_61 = env
-in {curmodule = _63_61.curmodule; curmonad = _63_61.curmonad; modules = _63_61.modules; open_namespaces = _63_61.open_namespaces; modul_abbrevs = _63_61.modul_abbrevs; sigaccum = _63_61.sigaccum; localbindings = _63_61.localbindings; recbindings = _63_61.recbindings; sigmap = _63_61.sigmap; default_result_effect = FStar_Syntax_Const.effect_Tot_lid; iface = _63_61.iface; admitted_iface = _63_61.admitted_iface; expect_typ = _63_61.expect_typ}))
+let _63_88 = env
+in {curmodule = _63_88.curmodule; curmonad = _63_88.curmonad; modules = _63_88.modules; scope_mods = _63_88.scope_mods; sigaccum = _63_88.sigaccum; sigmap = _63_88.sigmap; default_result_effect = FStar_Syntax_Const.effect_Tot_lid; iface = _63_88.iface; admitted_iface = _63_88.admitted_iface; expect_typ = _63_88.expect_typ}))
 
 
 let default_ml : env  ->  env = (fun env -> if (has_all_in_scope env) then begin
 (
 
-let _63_64 = env
-in {curmodule = _63_64.curmodule; curmonad = _63_64.curmonad; modules = _63_64.modules; open_namespaces = _63_64.open_namespaces; modul_abbrevs = _63_64.modul_abbrevs; sigaccum = _63_64.sigaccum; localbindings = _63_64.localbindings; recbindings = _63_64.recbindings; sigmap = _63_64.sigmap; default_result_effect = FStar_Syntax_Const.effect_ML_lid; iface = _63_64.iface; admitted_iface = _63_64.admitted_iface; expect_typ = _63_64.expect_typ})
+let _63_91 = env
+in {curmodule = _63_91.curmodule; curmonad = _63_91.curmonad; modules = _63_91.modules; scope_mods = _63_91.scope_mods; sigaccum = _63_91.sigaccum; sigmap = _63_91.sigmap; default_result_effect = FStar_Syntax_Const.effect_ML_lid; iface = _63_91.iface; admitted_iface = _63_91.admitted_iface; expect_typ = _63_91.expect_typ})
 end else begin
 env
 end)
@@ -119,12 +257,12 @@ let set_bv_range : FStar_Syntax_Syntax.bv  ->  FStar_Range.range  ->  FStar_Synt
 
 let id = (
 
-let _63_68 = bv.FStar_Syntax_Syntax.ppname
-in {FStar_Ident.idText = _63_68.FStar_Ident.idText; FStar_Ident.idRange = r})
+let _63_95 = bv.FStar_Syntax_Syntax.ppname
+in {FStar_Ident.idText = _63_95.FStar_Ident.idText; FStar_Ident.idRange = r})
 in (
 
-let _63_71 = bv
-in {FStar_Syntax_Syntax.ppname = id; FStar_Syntax_Syntax.index = _63_71.FStar_Syntax_Syntax.index; FStar_Syntax_Syntax.sort = _63_71.FStar_Syntax_Syntax.sort})))
+let _63_98 = bv
+in {FStar_Syntax_Syntax.ppname = id; FStar_Syntax_Syntax.index = _63_98.FStar_Syntax_Syntax.index; FStar_Syntax_Syntax.sort = _63_98.FStar_Syntax_Syntax.sort})))
 
 
 let bv_to_name : FStar_Syntax_Syntax.bv  ->  FStar_Range.range  ->  FStar_Syntax_Syntax.term = (fun bv r -> (FStar_Syntax_Syntax.bv_to_name (set_bv_range bv r)))
@@ -133,123 +271,319 @@ let bv_to_name : FStar_Syntax_Syntax.bv  ->  FStar_Range.range  ->  FStar_Syntax
 let unmangleMap : (Prims.string * Prims.string * FStar_Syntax_Syntax.delta_depth * FStar_Syntax_Syntax.fv_qual Prims.option) Prims.list = ((("op_ColonColon"), ("Cons"), (FStar_Syntax_Syntax.Delta_constant), (Some (FStar_Syntax_Syntax.Data_ctor))))::((("not"), ("op_Negation"), (FStar_Syntax_Syntax.Delta_equational), (None)))::[]
 
 
-let unmangleOpName : FStar_Ident.ident  ->  FStar_Syntax_Syntax.term Prims.option = (fun id -> (FStar_Util.find_map unmangleMap (fun _63_80 -> (match (_63_80) with
+let unmangleOpName : FStar_Ident.ident  ->  (FStar_Syntax_Syntax.term * Prims.bool) Prims.option = (fun id -> (
+
+let t = (FStar_Util.find_map unmangleMap (fun _63_107 -> (match (_63_107) with
 | (x, y, dd, dq) -> begin
 if (id.FStar_Ident.idText = x) then begin
-(let _158_123 = (let _158_122 = (FStar_Ident.lid_of_path (("Prims")::(y)::[]) id.FStar_Ident.idRange)
-in (FStar_Syntax_Syntax.fvar _158_122 dd dq))
-in Some (_158_123))
+(let _158_200 = (let _158_199 = (FStar_Ident.lid_of_path (("Prims")::(y)::[]) id.FStar_Ident.idRange)
+in (FStar_Syntax_Syntax.fvar _158_199 dd dq))
+in Some (_158_200))
 end else begin
 None
 end
-end))))
+end)))
+in (match (t) with
+| Some (v) -> begin
+Some (((v), (false)))
+end
+| None -> begin
+None
+end)))
+
+
+type 'a cont_t =
+| Cont_ok of 'a
+| Cont_fail
+| Cont_ignore
+
+
+let is_Cont_ok = (fun _ _discr_ -> (match (_discr_) with
+| Cont_ok (_) -> begin
+true
+end
+| _ -> begin
+false
+end))
+
+
+let is_Cont_fail = (fun _ _discr_ -> (match (_discr_) with
+| Cont_fail (_) -> begin
+true
+end
+| _ -> begin
+false
+end))
+
+
+let is_Cont_ignore = (fun _ _discr_ -> (match (_discr_) with
+| Cont_ignore (_) -> begin
+true
+end
+| _ -> begin
+false
+end))
+
+
+let ___Cont_ok____0 = (fun projectee -> (match (projectee) with
+| Cont_ok (_63_115) -> begin
+_63_115
+end))
+
+
+let option_of_cont = (fun k_ignore _63_1 -> (match (_63_1) with
+| Cont_ok (a) -> begin
+Some (a)
+end
+| Cont_fail -> begin
+None
+end
+| Cont_ignore -> begin
+(k_ignore ())
+end))
+
+
+let find_in_record = (fun ns id record cont -> (
+
+let needs_constrname = (not ((FStar_Syntax_Util.field_projector_contains_constructor id.FStar_Ident.idText)))
+in (
+
+let constrname = record.constrname.FStar_Ident.ident
+in (
+
+let fname = if needs_constrname then begin
+(let _158_231 = (FStar_Ident.lid_of_ids (FStar_List.append ns ((constrname)::[])))
+in (FStar_Syntax_Util.mk_field_projector_name_from_ident _158_231 id))
+end else begin
+(FStar_Ident.lid_of_ids (FStar_List.append ns ((id)::[])))
+end
+in (
+
+let fname = (FStar_Ident.set_lid_range fname id.FStar_Ident.idRange)
+in (
+
+let find = (FStar_Util.find_map record.fields (fun _63_134 -> (match (_63_134) with
+| (f, _63_133) -> begin
+if (FStar_Ident.lid_equals fname f) then begin
+Some (((record), (fname)))
+end else begin
+None
+end
+end)))
+in (match (find) with
+| Some (r) -> begin
+(cont r)
+end
+| None -> begin
+Cont_ignore
+end)))))))
+
+
+let try_lookup_id'' = (fun env id k_local_binding k_rec_binding k_record find_in_module lookup_default_id -> (
+
+let check_local_binding_id = (fun _63_2 -> (match (_63_2) with
+| (id', _63_150, _63_152) -> begin
+(id'.FStar_Ident.idText = id.FStar_Ident.idText)
+end))
+in (
+
+let check_rec_binding_id = (fun _63_3 -> (match (_63_3) with
+| (id', _63_158, _63_160) -> begin
+(id'.FStar_Ident.idText = id.FStar_Ident.idText)
+end))
+in (
+
+let curmod_ns = (let _158_262 = (current_module env)
+in (FStar_Ident.ids_of_lid _158_262))
+in (
+
+let proc = (fun _63_4 -> (match (_63_4) with
+| Local_binding (l) when (check_local_binding_id l) -> begin
+(k_local_binding l)
+end
+| Rec_binding (r) when (check_rec_binding_id r) -> begin
+(k_rec_binding r)
+end
+| Open_module_or_namespace (ns, _63_171) -> begin
+(
+
+let lid = (qual ns id)
+in (find_in_module lid))
+end
+| Top_level_def (id') when (id'.FStar_Ident.idText = id.FStar_Ident.idText) -> begin
+(lookup_default_id Cont_ignore id)
+end
+| Record_or_dc (r) -> begin
+(find_in_record curmod_ns id r k_record)
+end
+| _63_180 -> begin
+Cont_ignore
+end))
+in (
+
+let rec aux = (fun _63_5 -> (match (_63_5) with
+| (a)::q -> begin
+(let _158_268 = (proc a)
+in (option_of_cont (fun _63_187 -> (aux q)) _158_268))
+end
+| [] -> begin
+(let _158_270 = (lookup_default_id Cont_fail id)
+in (option_of_cont (fun _63_190 -> None) _158_270))
+end))
+in (aux env.scope_mods)))))))
+
+
+let found_local_binding = (fun _63_195 -> (match (_63_195) with
+| (id', x, mut) -> begin
+(let _158_272 = (bv_to_name x id'.FStar_Ident.idRange)
+in ((_158_272), (mut)))
+end))
+
+
+let find_in_module = (fun env lid k_global_def k_not_found -> (match ((FStar_Util.smap_try_find (sigmap env) lid.FStar_Ident.str)) with
+| Some (sb) -> begin
+(k_global_def lid sb)
+end
+| None -> begin
+k_not_found
+end))
 
 
 let try_lookup_id : env  ->  FStar_Ident.ident  ->  (FStar_Syntax_Syntax.term * Prims.bool) Prims.option = (fun env id -> (match ((unmangleOpName id)) with
 | Some (f) -> begin
-Some (((f), (false)))
+Some (f)
 end
-| _63_86 -> begin
-(FStar_Util.find_map env.localbindings (fun _63_1 -> (match (_63_1) with
-| (id', x, mut) when (id'.FStar_Ident.idText = id.FStar_Ident.idText) -> begin
-(let _158_130 = (let _158_129 = (bv_to_name x id.FStar_Ident.idRange)
-in ((_158_129), (mut)))
-in Some (_158_130))
-end
-| _63_93 -> begin
-None
-end)))
+| _63_208 -> begin
+(try_lookup_id'' env id (fun r -> (let _158_288 = (found_local_binding r)
+in Cont_ok (_158_288))) (fun _63_220 -> Cont_fail) (fun _63_218 -> Cont_ignore) (fun i -> (find_in_module env i (fun _63_214 _63_216 -> Cont_fail) Cont_ignore)) (fun _63_209 _63_211 -> Cont_fail))
 end))
 
 
-let resolve_in_open_namespaces' = (fun env lid finder -> (
+let lookup_default_id = (fun env id k_global_def k_not_found -> (
 
-let aux = (fun namespaces -> (match ((finder lid)) with
-| Some (r) -> begin
-Some (r)
-end
-| _63_103 -> begin
+let find_in_monad = (match (env.curmonad) with
+| Some (_63_229) -> begin
 (
 
-let found_in_monad = (match (((lid.FStar_Ident.ns), (env.curmonad))) with
-| ([], Some (_63_106)) -> begin
-(let _158_139 = (qualify env lid.FStar_Ident.ident)
-in (finder _158_139))
+let lid = (qualify env id)
+in (match ((FStar_Util.smap_try_find (sigmap env) lid.FStar_Ident.str)) with
+| Some (r) -> begin
+(let _158_306 = (k_global_def lid r)
+in Some (_158_306))
 end
-| _63_110 -> begin
+| None -> begin
+None
+end))
+end
+| None -> begin
 None
 end)
-in (match (found_in_monad) with
+in (match (find_in_monad) with
+| Some (v) -> begin
+v
+end
 | None -> begin
 (
 
-let ids = (FStar_Ident.ids_of_lid lid)
-in (FStar_Util.find_map namespaces (fun ns -> (
+let lid = (let _158_307 = (current_module env)
+in (qual _158_307 id))
+in (find_in_module env lid k_global_def k_not_found))
+end)))
 
-let full_name = (FStar_Ident.lid_of_ids (FStar_List.append (FStar_Ident.ids_of_lid ns) ids))
-in (finder full_name)))))
+
+let module_is_defined : env  ->  FStar_Ident.lident  ->  Prims.bool = (fun env lid -> ((let _158_312 = (current_module env)
+in (FStar_Ident.lid_equals lid _158_312)) || (FStar_List.existsb (fun x -> (FStar_Ident.lid_equals lid (Prims.fst x))) env.modules)))
+
+
+let resolve_module_name : env  ->  FStar_Ident.lident  ->  FStar_Ident.lident Prims.option = (fun env lid -> (
+
+let nslen = (FStar_List.length lid.FStar_Ident.ns)
+in (
+
+let rec aux = (fun _63_6 -> (match (_63_6) with
+| [] -> begin
+if (module_is_defined env lid) then begin
+Some (lid)
+end else begin
+None
 end
-| x -> begin
-x
+end
+| (Open_module_or_namespace (ns, Open_namespace))::q -> begin
+(
+
+let new_lid = (let _158_322 = (let _158_321 = (FStar_Ident.path_of_lid ns)
+in (let _158_320 = (FStar_Ident.path_of_lid lid)
+in (FStar_List.append _158_321 _158_320)))
+in (FStar_Ident.lid_of_path _158_322 (FStar_Ident.range_of_lid lid)))
+in if (module_is_defined env new_lid) then begin
+Some (new_lid)
+end else begin
+(aux q)
+end)
+end
+| (Module_abbrev (name, modul))::_63_258 when ((nslen = (Prims.parse_int "0")) && (name.FStar_Ident.idText = lid.FStar_Ident.ident.FStar_Ident.idText)) -> begin
+Some (modul)
+end
+| (_63_266)::q -> begin
+(aux q)
 end))
-end))
-in (let _158_142 = (let _158_141 = (current_module env)
-in (_158_141)::env.open_namespaces)
-in (aux _158_142))))
+in (aux env.scope_mods))))
 
 
-let expand_module_abbrev : env  ->  FStar_Ident.lident  ->  FStar_Ident.lident = (fun env lid -> (match (lid.FStar_Ident.ns) with
-| (_63_122)::_63_120 -> begin
-lid
+let resolve_in_open_namespaces'' = (fun env lid k_local_binding k_rec_binding k_record f_module l_default -> (match (lid.FStar_Ident.ns) with
+| (_63_279)::_63_277 -> begin
+(match ((let _158_352 = (let _158_351 = (FStar_Ident.lid_of_ids lid.FStar_Ident.ns)
+in (FStar_Ident.set_lid_range _158_351 (FStar_Ident.range_of_lid lid)))
+in (resolve_module_name env _158_352))) with
+| None -> begin
+None
+end
+| Some (modul) -> begin
+(
+
+let lid' = (qual modul lid.FStar_Ident.ident)
+in (let _158_354 = (f_module Cont_fail lid')
+in (option_of_cont (fun _63_285 -> None) _158_354)))
+end)
 end
 | [] -> begin
+(try_lookup_id'' env lid.FStar_Ident.ident k_local_binding k_rec_binding k_record (f_module Cont_ignore) l_default)
+end))
+
+
+let cont_of_option = (fun k_none _63_7 -> (match (_63_7) with
+| Some (v) -> begin
+Cont_ok (v)
+end
+| None -> begin
+k_none
+end))
+
+
+let resolve_in_open_namespaces' = (fun env lid k_local_binding k_rec_binding k_global_def -> (
+
+let k_global_def' = (fun k lid def -> (let _158_380 = (k_global_def lid def)
+in (cont_of_option k _158_380)))
+in (
+
+let f_module = (fun k lid' -> (find_in_module env lid' (k_global_def' k) k))
+in (
+
+let l_default = (fun k i -> (lookup_default_id env i (k_global_def' k) k))
+in (resolve_in_open_namespaces'' env lid (fun l -> (let _158_390 = (k_local_binding l)
+in (cont_of_option Cont_fail _158_390))) (fun r -> (let _158_392 = (k_rec_binding r)
+in (cont_of_option Cont_fail _158_392))) (fun _63_310 -> Cont_ignore) f_module l_default)))))
+
+
+let fv_qual_of_se : FStar_Syntax_Syntax.sigelt  ->  FStar_Syntax_Syntax.fv_qual Prims.option = (fun _63_9 -> (match (_63_9) with
+| FStar_Syntax_Syntax.Sig_datacon (_63_316, _63_318, _63_320, l, _63_323, quals, _63_326, _63_328) -> begin
 (
 
-let id = lid.FStar_Ident.ident
-in (match ((FStar_List.tryFind (fun _63_129 -> (match (_63_129) with
-| (id', _63_128) -> begin
-(id.FStar_Ident.idText = id'.FStar_Ident.idText)
-end)) env.modul_abbrevs)) with
-| None -> begin
-lid
-end
-| Some (_63_132, lid') -> begin
-lid'
-end))
-end))
-
-
-let expand_module_abbrevs : env  ->  FStar_Ident.lident  ->  FStar_Ident.lident = (fun env lid -> (match (lid.FStar_Ident.ns) with
-| (id)::rest -> begin
-(match ((FStar_All.pipe_right env.modul_abbrevs (FStar_List.tryFind (fun _63_144 -> (match (_63_144) with
-| (id', _63_143) -> begin
-(id.FStar_Ident.idText = id'.FStar_Ident.idText)
-end))))) with
-| None -> begin
-lid
-end
-| Some (_63_147, lid') -> begin
-(FStar_Ident.lid_of_ids (FStar_List.append (FStar_Ident.ids_of_lid lid') (FStar_List.append rest ((lid.FStar_Ident.ident)::[]))))
-end)
-end
-| _63_152 -> begin
-lid
-end))
-
-
-let resolve_in_open_namespaces = (fun env lid finder -> (let _158_159 = (expand_module_abbrevs env lid)
-in (resolve_in_open_namespaces' env _158_159 finder)))
-
-
-let fv_qual_of_se : FStar_Syntax_Syntax.sigelt  ->  FStar_Syntax_Syntax.fv_qual Prims.option = (fun _63_3 -> (match (_63_3) with
-| FStar_Syntax_Syntax.Sig_datacon (_63_159, _63_161, _63_163, l, _63_166, quals, _63_169, _63_171) -> begin
-(
-
-let qopt = (FStar_Util.find_map quals (fun _63_2 -> (match (_63_2) with
+let qopt = (FStar_Util.find_map quals (fun _63_8 -> (match (_63_8) with
 | FStar_Syntax_Syntax.RecordConstructor (fs) -> begin
 Some (FStar_Syntax_Syntax.Record_ctor (((l), (fs))))
 end
-| _63_178 -> begin
+| _63_335 -> begin
 None
 end)))
 in (match (qopt) with
@@ -260,15 +594,15 @@ end
 x
 end))
 end
-| FStar_Syntax_Syntax.Sig_declare_typ (_63_183, _63_185, _63_187, quals, _63_190) -> begin
+| FStar_Syntax_Syntax.Sig_declare_typ (_63_340, _63_342, _63_344, quals, _63_347) -> begin
 None
 end
-| _63_194 -> begin
+| _63_351 -> begin
 None
 end))
 
 
-let lb_fv : FStar_Syntax_Syntax.letbinding Prims.list  ->  FStar_Ident.lident  ->  FStar_Syntax_Syntax.fv = (fun lbs lid -> (let _158_168 = (FStar_Util.find_map lbs (fun lb -> (
+let lb_fv : FStar_Syntax_Syntax.letbinding Prims.list  ->  FStar_Ident.lident  ->  FStar_Syntax_Syntax.fv = (fun lbs lid -> (let _158_402 = (FStar_Util.find_map lbs (fun lb -> (
 
 let fv = (FStar_Util.right lb.FStar_Syntax_Syntax.lbname)
 in if (FStar_Syntax_Syntax.fv_eq_lid fv lid) then begin
@@ -276,11 +610,11 @@ Some (fv)
 end else begin
 None
 end)))
-in (FStar_All.pipe_right _158_168 FStar_Util.must)))
+in (FStar_All.pipe_right _158_402 FStar_Util.must)))
 
 
-let ns_of_lid_equals : FStar_Ident.lident  ->  FStar_Ident.lident  ->  Prims.bool = (fun lid ns -> (((FStar_List.length lid.FStar_Ident.ns) = (FStar_List.length (FStar_Ident.ids_of_lid ns))) && (let _158_173 = (FStar_Ident.lid_of_ids lid.FStar_Ident.ns)
-in (FStar_Ident.lid_equals _158_173 ns))))
+let ns_of_lid_equals : FStar_Ident.lident  ->  FStar_Ident.lident  ->  Prims.bool = (fun lid ns -> (((FStar_List.length lid.FStar_Ident.ns) = (FStar_List.length (FStar_Ident.ids_of_lid ns))) && (let _158_407 = (FStar_Ident.lid_of_ids lid.FStar_Ident.ns)
+in (FStar_Ident.lid_equals _158_407 ns))))
 
 
 let try_lookup_name : Prims.bool  ->  Prims.bool  ->  env  ->  FStar_Ident.lident  ->  foundname Prims.option = (fun any_val exclude_interf env lid -> (
@@ -288,43 +622,40 @@ let try_lookup_name : Prims.bool  ->  Prims.bool  ->  env  ->  FStar_Ident.liden
 let occurrence_range = (FStar_Ident.range_of_lid lid)
 in (
 
-let find_in_sig = (fun source_lid -> (match ((FStar_Util.smap_try_find (sigmap env) source_lid.FStar_Ident.str)) with
-| Some (_63_209, true) when exclude_interf -> begin
+let k_global_def = (fun source_lid _63_13 -> (match (_63_13) with
+| (_63_367, true) when exclude_interf -> begin
 None
 end
-| None -> begin
-None
-end
-| Some (se, _63_216) -> begin
+| (se, _63_372) -> begin
 (match (se) with
-| FStar_Syntax_Syntax.Sig_inductive_typ (_63_220) -> begin
-(let _158_186 = (let _158_185 = (let _158_184 = (FStar_Syntax_Syntax.fvar source_lid FStar_Syntax_Syntax.Delta_constant None)
-in ((_158_184), (false)))
-in Term_name (_158_185))
-in Some (_158_186))
+| FStar_Syntax_Syntax.Sig_inductive_typ (_63_375) -> begin
+(let _158_422 = (let _158_421 = (let _158_420 = (FStar_Syntax_Syntax.fvar source_lid FStar_Syntax_Syntax.Delta_constant None)
+in ((_158_420), (false)))
+in Term_name (_158_421))
+in Some (_158_422))
 end
-| FStar_Syntax_Syntax.Sig_datacon (_63_223) -> begin
-(let _158_190 = (let _158_189 = (let _158_188 = (let _158_187 = (fv_qual_of_se se)
-in (FStar_Syntax_Syntax.fvar source_lid FStar_Syntax_Syntax.Delta_constant _158_187))
-in ((_158_188), (false)))
-in Term_name (_158_189))
-in Some (_158_190))
+| FStar_Syntax_Syntax.Sig_datacon (_63_378) -> begin
+(let _158_426 = (let _158_425 = (let _158_424 = (let _158_423 = (fv_qual_of_se se)
+in (FStar_Syntax_Syntax.fvar source_lid FStar_Syntax_Syntax.Delta_constant _158_423))
+in ((_158_424), (false)))
+in Term_name (_158_425))
+in Some (_158_426))
 end
-| FStar_Syntax_Syntax.Sig_let ((_63_226, lbs), _63_230, _63_232, _63_234) -> begin
+| FStar_Syntax_Syntax.Sig_let ((_63_381, lbs), _63_385, _63_387, _63_389) -> begin
 (
 
 let fv = (lb_fv lbs source_lid)
-in (let _158_193 = (let _158_192 = (let _158_191 = (FStar_Syntax_Syntax.fvar source_lid fv.FStar_Syntax_Syntax.fv_delta fv.FStar_Syntax_Syntax.fv_qual)
-in ((_158_191), (false)))
-in Term_name (_158_192))
-in Some (_158_193)))
+in (let _158_429 = (let _158_428 = (let _158_427 = (FStar_Syntax_Syntax.fvar source_lid fv.FStar_Syntax_Syntax.fv_delta fv.FStar_Syntax_Syntax.fv_qual)
+in ((_158_427), (false)))
+in Term_name (_158_428))
+in Some (_158_429)))
 end
-| FStar_Syntax_Syntax.Sig_declare_typ (lid, _63_240, _63_242, quals, _63_245) -> begin
-if (any_val || (FStar_All.pipe_right quals (FStar_Util.for_some (fun _63_4 -> (match (_63_4) with
+| FStar_Syntax_Syntax.Sig_declare_typ (lid, _63_395, _63_397, quals, _63_400) -> begin
+if (any_val || (FStar_All.pipe_right quals (FStar_Util.for_some (fun _63_10 -> (match (_63_10) with
 | FStar_Syntax_Syntax.Assumption -> begin
 true
 end
-| _63_251 -> begin
+| _63_406 -> begin
 false
 end))))) then begin
 (
@@ -332,22 +663,22 @@ end))))) then begin
 let lid = (FStar_Ident.set_lid_range lid (FStar_Ident.range_of_lid source_lid))
 in (
 
-let dd = if ((FStar_Syntax_Util.is_primop_lid lid) || ((ns_of_lid_equals lid FStar_Syntax_Const.prims_lid) && (FStar_All.pipe_right quals (FStar_Util.for_some (fun _63_5 -> (match (_63_5) with
+let dd = if ((FStar_Syntax_Util.is_primop_lid lid) || ((ns_of_lid_equals lid FStar_Syntax_Const.prims_lid) && (FStar_All.pipe_right quals (FStar_Util.for_some (fun _63_11 -> (match (_63_11) with
 | (FStar_Syntax_Syntax.Projector (_)) | (FStar_Syntax_Syntax.Discriminator (_)) -> begin
 true
 end
-| _63_261 -> begin
+| _63_416 -> begin
 false
 end)))))) then begin
 FStar_Syntax_Syntax.Delta_equational
 end else begin
 FStar_Syntax_Syntax.Delta_constant
 end
-in (match ((FStar_Util.find_map quals (fun _63_6 -> (match (_63_6) with
+in (match ((FStar_Util.find_map quals (fun _63_12 -> (match (_63_12) with
 | FStar_Syntax_Syntax.Reflectable (refl_monad) -> begin
 Some (refl_monad)
 end
-| _63_267 -> begin
+| _63_422 -> begin
 None
 end)))) with
 | Some (refl_monad) -> begin
@@ -356,12 +687,12 @@ end)))) with
 let refl_const = (FStar_Syntax_Syntax.mk (FStar_Syntax_Syntax.Tm_constant (FStar_Const.Const_reflect (refl_monad))) None occurrence_range)
 in Some (Term_name (((refl_const), (false)))))
 end
-| _63_272 -> begin
-(let _158_200 = (let _158_199 = (let _158_198 = (let _158_197 = (fv_qual_of_se se)
-in (FStar_Syntax_Syntax.fvar lid dd _158_197))
-in ((_158_198), (false)))
-in Term_name (_158_199))
-in Some (_158_200))
+| _63_427 -> begin
+(let _158_436 = (let _158_435 = (let _158_434 = (let _158_433 = (fv_qual_of_se se)
+in (FStar_Syntax_Syntax.fvar lid dd _158_433))
+in ((_158_434), (false)))
+in Term_name (_158_435))
+in Some (_158_436))
 end)))
 end else begin
 None
@@ -370,55 +701,56 @@ end
 | (FStar_Syntax_Syntax.Sig_new_effect_for_free (ne, _)) | (FStar_Syntax_Syntax.Sig_new_effect (ne, _)) -> begin
 Some (Eff_name (((se), ((FStar_Ident.set_lid_range ne.FStar_Syntax_Syntax.mname (FStar_Ident.range_of_lid source_lid))))))
 end
-| FStar_Syntax_Syntax.Sig_effect_abbrev (_63_283) -> begin
+| FStar_Syntax_Syntax.Sig_effect_abbrev (_63_438) -> begin
 Some (Eff_name (((se), (source_lid))))
 end
-| _63_286 -> begin
+| _63_441 -> begin
 None
 end)
 end))
 in (
 
-let found_id = (match (lid.FStar_Ident.ns) with
-| [] -> begin
-(match ((try_lookup_id env lid.FStar_Ident.ident)) with
-| Some (e, mut) -> begin
-Some (Term_name (((e), (mut))))
-end
-| None -> begin
-(
+let k_local_binding = (fun r -> (let _158_440 = (let _158_439 = (found_local_binding r)
+in Term_name (_158_439))
+in Some (_158_440)))
+in (
 
-let recname = (qualify env lid.FStar_Ident.ident)
-in (FStar_Util.find_map env.recbindings (fun _63_297 -> (match (_63_297) with
+let k_rec_binding = (fun _63_448 -> (match (_63_448) with
 | (id, l, dd) -> begin
-if (id.FStar_Ident.idText = lid.FStar_Ident.ident.FStar_Ident.idText) then begin
-(let _158_204 = (let _158_203 = (let _158_202 = (FStar_Syntax_Syntax.fvar (FStar_Ident.set_lid_range l (FStar_Ident.range_of_lid lid)) dd None)
-in ((_158_202), (false)))
-in Term_name (_158_203))
-in Some (_158_204))
-end else begin
-None
+(let _158_445 = (let _158_444 = (let _158_443 = (FStar_Syntax_Syntax.fvar (FStar_Ident.set_lid_range l (FStar_Ident.range_of_lid lid)) dd None)
+in ((_158_443), (false)))
+in Term_name (_158_444))
+in Some (_158_445))
+end))
+in (
+
+let found_unmangled = (match (lid.FStar_Ident.ns) with
+| [] -> begin
+(match ((unmangleOpName lid.FStar_Ident.ident)) with
+| Some (f) -> begin
+Some (Term_name (f))
 end
-end))))
+| _63_453 -> begin
+None
 end)
 end
-| _63_299 -> begin
+| _63_455 -> begin
 None
 end)
-in (match (found_id) with
-| Some (_63_302) -> begin
-found_id
+in (match (found_unmangled) with
+| None -> begin
+(resolve_in_open_namespaces' env lid k_local_binding k_rec_binding k_global_def)
 end
-| _63_305 -> begin
-(resolve_in_open_namespaces env lid find_in_sig)
-end)))))
+| x -> begin
+x
+end)))))))
 
 
 let try_lookup_effect_name' : Prims.bool  ->  env  ->  FStar_Ident.lident  ->  (FStar_Syntax_Syntax.sigelt * FStar_Ident.lident) Prims.option = (fun exclude_interf env lid -> (match ((try_lookup_name true exclude_interf env lid)) with
 | Some (Eff_name (o, l)) -> begin
 Some (((o), (l)))
 end
-| _63_315 -> begin
+| _63_468 -> begin
 None
 end))
 
@@ -427,19 +759,19 @@ let try_lookup_effect_name : env  ->  FStar_Ident.lident  ->  FStar_Ident.lident
 | Some (o, l) -> begin
 Some (l)
 end
-| _63_323 -> begin
+| _63_476 -> begin
 None
 end))
 
 
 let try_lookup_effect_defn : env  ->  FStar_Ident.lident  ->  FStar_Syntax_Syntax.eff_decl Prims.option = (fun env l -> (match ((try_lookup_effect_name' (not (env.iface)) env l)) with
-| Some (FStar_Syntax_Syntax.Sig_new_effect (ne, _63_328), _63_332) -> begin
+| Some (FStar_Syntax_Syntax.Sig_new_effect (ne, _63_481), _63_485) -> begin
 Some (ne)
 end
-| Some (FStar_Syntax_Syntax.Sig_new_effect_for_free (ne, _63_337), _63_341) -> begin
+| Some (FStar_Syntax_Syntax.Sig_new_effect_for_free (ne, _63_490), _63_494) -> begin
 Some (ne)
 end
-| _63_345 -> begin
+| _63_498 -> begin
 None
 end))
 
@@ -448,34 +780,34 @@ let is_effect_name : env  ->  FStar_Ident.lident  ->  Prims.bool = (fun env lid 
 | None -> begin
 false
 end
-| Some (_63_350) -> begin
+| Some (_63_503) -> begin
 true
 end))
 
 
 let lookup_letbinding_quals : env  ->  FStar_Ident.lident  ->  FStar_Syntax_Syntax.qualifier Prims.list = (fun env lid -> (
 
-let find_in_sig = (fun lid -> (match ((FStar_Util.smap_try_find (sigmap env) lid.FStar_Ident.str)) with
-| Some (FStar_Syntax_Syntax.Sig_declare_typ (lid, _63_358, _63_360, quals, _63_363), _63_367) -> begin
+let k_global_def = (fun lid _63_14 -> (match (_63_14) with
+| (FStar_Syntax_Syntax.Sig_declare_typ (lid, _63_512, _63_514, quals, _63_517), _63_521) -> begin
 Some (quals)
 end
-| _63_371 -> begin
+| _63_524 -> begin
 None
 end))
-in (match ((resolve_in_open_namespaces env lid find_in_sig)) with
+in (match ((resolve_in_open_namespaces' env lid (fun _63_527 -> None) (fun _63_525 -> None) k_global_def)) with
 | Some (quals) -> begin
 quals
 end
-| _63_375 -> begin
+| _63_532 -> begin
 []
 end)))
 
 
-let try_lookup_module : env  ->  Prims.string Prims.list  ->  FStar_Syntax_Syntax.modul Prims.option = (fun env path -> (match ((FStar_List.tryFind (fun _63_380 -> (match (_63_380) with
+let try_lookup_module : env  ->  Prims.string Prims.list  ->  FStar_Syntax_Syntax.modul Prims.option = (fun env path -> (match ((FStar_List.tryFind (fun _63_537 -> (match (_63_537) with
 | (mlid, modul) -> begin
 ((FStar_Ident.path_of_lid mlid) = path)
 end)) env.modules)) with
-| Some (_63_382, modul) -> begin
+| Some (_63_539, modul) -> begin
 Some (modul)
 end
 | None -> begin
@@ -485,43 +817,43 @@ end))
 
 let try_lookup_let : env  ->  FStar_Ident.lident  ->  FStar_Syntax_Syntax.term Prims.option = (fun env lid -> (
 
-let find_in_sig = (fun lid -> (match ((FStar_Util.smap_try_find (sigmap env) lid.FStar_Ident.str)) with
-| Some (FStar_Syntax_Syntax.Sig_let ((_63_392, lbs), _63_396, _63_398, _63_400), _63_404) -> begin
+let k_global_def = (fun lid _63_15 -> (match (_63_15) with
+| (FStar_Syntax_Syntax.Sig_let ((_63_550, lbs), _63_554, _63_556, _63_558), _63_562) -> begin
 (
 
 let fv = (lb_fv lbs lid)
-in (let _158_240 = (FStar_Syntax_Syntax.fvar lid fv.FStar_Syntax_Syntax.fv_delta fv.FStar_Syntax_Syntax.fv_qual)
-in Some (_158_240)))
+in (let _158_487 = (FStar_Syntax_Syntax.fvar lid fv.FStar_Syntax_Syntax.fv_delta fv.FStar_Syntax_Syntax.fv_qual)
+in Some (_158_487)))
 end
-| _63_409 -> begin
+| _63_566 -> begin
 None
 end))
-in (resolve_in_open_namespaces env lid find_in_sig)))
+in (resolve_in_open_namespaces' env lid (fun _63_569 -> None) (fun _63_567 -> None) k_global_def)))
 
 
 let try_lookup_definition : env  ->  FStar_Ident.lident  ->  FStar_Syntax_Syntax.term Prims.option = (fun env lid -> (
 
-let find_in_sig = (fun lid -> (match ((FStar_Util.smap_try_find (sigmap env) lid.FStar_Ident.str)) with
-| Some (FStar_Syntax_Syntax.Sig_let (lbs, _63_416, _63_418, _63_420), _63_424) -> begin
+let k_global_def = (fun lid _63_16 -> (match (_63_16) with
+| (FStar_Syntax_Syntax.Sig_let (lbs, _63_578, _63_580, _63_582), _63_586) -> begin
 (FStar_Util.find_map (Prims.snd lbs) (fun lb -> (match (lb.FStar_Syntax_Syntax.lbname) with
 | FStar_Util.Inr (fv) when (FStar_Syntax_Syntax.fv_eq_lid fv lid) -> begin
 Some (lb.FStar_Syntax_Syntax.lbdef)
 end
-| _63_431 -> begin
+| _63_592 -> begin
 None
 end)))
 end
-| _63_433 -> begin
+| _63_594 -> begin
 None
 end))
-in (resolve_in_open_namespaces env lid find_in_sig)))
+in (resolve_in_open_namespaces' env lid (fun _63_597 -> None) (fun _63_595 -> None) k_global_def)))
 
 
 let try_lookup_lid' : Prims.bool  ->  Prims.bool  ->  env  ->  FStar_Ident.lident  ->  (FStar_Syntax_Syntax.term * Prims.bool) Prims.option = (fun any_val exclude_interf env lid -> (match ((try_lookup_name any_val exclude_interf env lid)) with
 | Some (Term_name (e, mut)) -> begin
 Some (((e), (mut)))
 end
-| _63_444 -> begin
+| _63_609 -> begin
 None
 end))
 
@@ -531,41 +863,41 @@ let try_lookup_lid : env  ->  FStar_Ident.lident  ->  (FStar_Syntax_Syntax.term 
 
 let try_lookup_datacon : env  ->  FStar_Ident.lident  ->  FStar_Syntax_Syntax.fv Prims.option = (fun env lid -> (
 
-let find_in_sig = (fun lid -> (match ((FStar_Util.smap_try_find (sigmap env) lid.FStar_Ident.str)) with
-| Some (FStar_Syntax_Syntax.Sig_declare_typ (_63_452, _63_454, _63_456, quals, _63_459), _63_463) -> begin
-if (FStar_All.pipe_right quals (FStar_Util.for_some (fun _63_7 -> (match (_63_7) with
+let k_global_def = (fun lid _63_18 -> (match (_63_18) with
+| (FStar_Syntax_Syntax.Sig_declare_typ (_63_618, _63_620, _63_622, quals, _63_625), _63_629) -> begin
+if (FStar_All.pipe_right quals (FStar_Util.for_some (fun _63_17 -> (match (_63_17) with
 | FStar_Syntax_Syntax.Assumption -> begin
 true
 end
-| _63_469 -> begin
+| _63_634 -> begin
 false
 end)))) then begin
-(let _158_267 = (FStar_Syntax_Syntax.lid_as_fv lid FStar_Syntax_Syntax.Delta_constant None)
-in Some (_158_267))
+(let _158_522 = (FStar_Syntax_Syntax.lid_as_fv lid FStar_Syntax_Syntax.Delta_constant None)
+in Some (_158_522))
 end else begin
 None
 end
 end
-| Some (FStar_Syntax_Syntax.Sig_datacon (_63_471), _63_474) -> begin
-(let _158_268 = (FStar_Syntax_Syntax.lid_as_fv lid FStar_Syntax_Syntax.Delta_constant (Some (FStar_Syntax_Syntax.Data_ctor)))
-in Some (_158_268))
+| (FStar_Syntax_Syntax.Sig_datacon (_63_636), _63_639) -> begin
+(let _158_523 = (FStar_Syntax_Syntax.lid_as_fv lid FStar_Syntax_Syntax.Delta_constant (Some (FStar_Syntax_Syntax.Data_ctor)))
+in Some (_158_523))
 end
-| _63_478 -> begin
+| _63_642 -> begin
 None
 end))
-in (resolve_in_open_namespaces env lid find_in_sig)))
+in (resolve_in_open_namespaces' env lid (fun _63_645 -> None) (fun _63_643 -> None) k_global_def)))
 
 
 let find_all_datacons : env  ->  FStar_Ident.lident  ->  FStar_Ident.lident Prims.list Prims.option = (fun env lid -> (
 
-let find_in_sig = (fun lid -> (match ((FStar_Util.smap_try_find (sigmap env) lid.FStar_Ident.str)) with
-| Some (FStar_Syntax_Syntax.Sig_inductive_typ (_63_484, _63_486, _63_488, _63_490, _63_492, datas, _63_495, _63_497), _63_501) -> begin
+let k_global_def = (fun lid _63_19 -> (match (_63_19) with
+| (FStar_Syntax_Syntax.Sig_inductive_typ (_63_653, _63_655, _63_657, _63_659, _63_661, datas, _63_664, _63_666), _63_670) -> begin
 Some (datas)
 end
-| _63_505 -> begin
+| _63_673 -> begin
 None
 end))
-in (resolve_in_open_namespaces env lid find_in_sig)))
+in (resolve_in_open_namespaces' env lid (fun _63_676 -> None) (fun _63_674 -> None) k_global_def)))
 
 
 let record_cache_aux : ((Prims.unit  ->  Prims.unit) * (Prims.unit  ->  Prims.unit) * (Prims.unit  ->  record_or_dc Prims.list) * (record_or_dc  ->  Prims.unit) * (Prims.unit  ->  Prims.unit)) = (
@@ -573,46 +905,46 @@ let record_cache_aux : ((Prims.unit  ->  Prims.unit) * (Prims.unit  ->  Prims.un
 let record_cache = (FStar_Util.mk_ref (([])::[]))
 in (
 
-let push = (fun _63_508 -> (match (()) with
+let push = (fun _63_680 -> (match (()) with
 | () -> begin
-(let _158_290 = (let _158_289 = (let _158_287 = (FStar_ST.read record_cache)
-in (FStar_List.hd _158_287))
-in (let _158_288 = (FStar_ST.read record_cache)
-in (_158_289)::_158_288))
-in (FStar_ST.op_Colon_Equals record_cache _158_290))
+(let _158_551 = (let _158_550 = (let _158_548 = (FStar_ST.read record_cache)
+in (FStar_List.hd _158_548))
+in (let _158_549 = (FStar_ST.read record_cache)
+in (_158_550)::_158_549))
+in (FStar_ST.op_Colon_Equals record_cache _158_551))
 end))
 in (
 
-let pop = (fun _63_510 -> (match (()) with
+let pop = (fun _63_682 -> (match (()) with
 | () -> begin
-(let _158_294 = (let _158_293 = (FStar_ST.read record_cache)
-in (FStar_List.tl _158_293))
-in (FStar_ST.op_Colon_Equals record_cache _158_294))
+(let _158_555 = (let _158_554 = (FStar_ST.read record_cache)
+in (FStar_List.tl _158_554))
+in (FStar_ST.op_Colon_Equals record_cache _158_555))
 end))
 in (
 
-let peek = (fun _63_512 -> (match (()) with
+let peek = (fun _63_684 -> (match (()) with
 | () -> begin
-(let _158_297 = (FStar_ST.read record_cache)
-in (FStar_List.hd _158_297))
+(let _158_558 = (FStar_ST.read record_cache)
+in (FStar_List.hd _158_558))
 end))
 in (
 
-let insert = (fun r -> (let _158_304 = (let _158_303 = (let _158_300 = (peek ())
-in (r)::_158_300)
-in (let _158_302 = (let _158_301 = (FStar_ST.read record_cache)
-in (FStar_List.tl _158_301))
-in (_158_303)::_158_302))
-in (FStar_ST.op_Colon_Equals record_cache _158_304)))
+let insert = (fun r -> (let _158_565 = (let _158_564 = (let _158_561 = (peek ())
+in (r)::_158_561)
+in (let _158_563 = (let _158_562 = (FStar_ST.read record_cache)
+in (FStar_List.tl _158_562))
+in (_158_564)::_158_563))
+in (FStar_ST.op_Colon_Equals record_cache _158_565)))
 in (
 
-let commit = (fun _63_516 -> (match (()) with
+let commit = (fun _63_688 -> (match (()) with
 | () -> begin
 (match ((FStar_ST.read record_cache)) with
-| (hd)::(_63_519)::tl -> begin
+| (hd)::(_63_691)::tl -> begin
 (FStar_ST.op_Colon_Equals record_cache ((hd)::tl))
 end
-| _63_524 -> begin
+| _63_696 -> begin
 (FStar_All.failwith "Impossible")
 end)
 end))
@@ -621,157 +953,149 @@ in ((push), (pop), (peek), (insert), (commit))))))))
 
 let push_record_cache : Prims.unit  ->  Prims.unit = (
 
-let _63_534 = record_cache_aux
-in (match (_63_534) with
-| (push, _63_527, _63_529, _63_531, _63_533) -> begin
+let _63_706 = record_cache_aux
+in (match (_63_706) with
+| (push, _63_699, _63_701, _63_703, _63_705) -> begin
 push
 end))
 
 
 let pop_record_cache : Prims.unit  ->  Prims.unit = (
 
-let _63_544 = record_cache_aux
-in (match (_63_544) with
-| (_63_536, pop, _63_539, _63_541, _63_543) -> begin
+let _63_716 = record_cache_aux
+in (match (_63_716) with
+| (_63_708, pop, _63_711, _63_713, _63_715) -> begin
 pop
 end))
 
 
 let peek_record_cache : Prims.unit  ->  record_or_dc Prims.list = (
 
-let _63_554 = record_cache_aux
-in (match (_63_554) with
-| (_63_546, _63_548, peek, _63_551, _63_553) -> begin
+let _63_726 = record_cache_aux
+in (match (_63_726) with
+| (_63_718, _63_720, peek, _63_723, _63_725) -> begin
 peek
 end))
 
 
 let insert_record_cache : record_or_dc  ->  Prims.unit = (
 
-let _63_564 = record_cache_aux
-in (match (_63_564) with
-| (_63_556, _63_558, _63_560, insert, _63_563) -> begin
+let _63_736 = record_cache_aux
+in (match (_63_736) with
+| (_63_728, _63_730, _63_732, insert, _63_735) -> begin
 insert
 end))
 
 
 let commit_record_cache : Prims.unit  ->  Prims.unit = (
 
-let _63_574 = record_cache_aux
-in (match (_63_574) with
-| (_63_566, _63_568, _63_570, _63_572, commit) -> begin
+let _63_746 = record_cache_aux
+in (match (_63_746) with
+| (_63_738, _63_740, _63_742, _63_744, commit) -> begin
 commit
 end))
 
 
-let extract_record : env  ->  FStar_Syntax_Syntax.sigelt  ->  Prims.unit = (fun e _63_11 -> (match (_63_11) with
-| FStar_Syntax_Syntax.Sig_bundle (sigs, _63_579, _63_581, _63_583) -> begin
+let extract_record : env  ->  scope_mod Prims.list FStar_ST.ref  ->  FStar_Syntax_Syntax.sigelt  ->  Prims.unit = (fun e new_globs _63_23 -> (match (_63_23) with
+| FStar_Syntax_Syntax.Sig_bundle (sigs, _63_752, _63_754, _63_756) -> begin
 (
 
-let is_rec = (FStar_Util.for_some (fun _63_8 -> (match (_63_8) with
+let is_rec = (FStar_Util.for_some (fun _63_20 -> (match (_63_20) with
 | (FStar_Syntax_Syntax.RecordType (_)) | (FStar_Syntax_Syntax.RecordConstructor (_)) -> begin
 true
 end
-| _63_594 -> begin
+| _63_767 -> begin
 false
 end)))
 in (
 
-let find_dc = (fun dc -> (FStar_All.pipe_right sigs (FStar_Util.find_opt (fun _63_9 -> (match (_63_9) with
-| FStar_Syntax_Syntax.Sig_datacon (lid, _63_601, _63_603, _63_605, _63_607, _63_609, _63_611, _63_613) -> begin
+let find_dc = (fun dc -> (FStar_All.pipe_right sigs (FStar_Util.find_opt (fun _63_21 -> (match (_63_21) with
+| FStar_Syntax_Syntax.Sig_datacon (lid, _63_774, _63_776, _63_778, _63_780, _63_782, _63_784, _63_786) -> begin
 (FStar_Ident.lid_equals dc lid)
 end
-| _63_617 -> begin
+| _63_790 -> begin
 false
 end)))))
-in (FStar_All.pipe_right sigs (FStar_List.iter (fun _63_10 -> (match (_63_10) with
-| FStar_Syntax_Syntax.Sig_inductive_typ (typename, univs, parms, _63_623, _63_625, (dc)::[], tags, _63_630) -> begin
-(match ((let _158_407 = (find_dc dc)
-in (FStar_All.pipe_left FStar_Util.must _158_407))) with
-| FStar_Syntax_Syntax.Sig_datacon (constrname, _63_635, t, _63_638, _63_640, _63_642, _63_644, _63_646) -> begin
+in (FStar_All.pipe_right sigs (FStar_List.iter (fun _63_22 -> (match (_63_22) with
+| FStar_Syntax_Syntax.Sig_inductive_typ (typename, univs, parms, _63_796, _63_798, (dc)::[], tags, _63_803) -> begin
+(match ((let _158_670 = (find_dc dc)
+in (FStar_All.pipe_left FStar_Util.must _158_670))) with
+| FStar_Syntax_Syntax.Sig_datacon (constrname, _63_808, t, _63_811, _63_813, _63_815, _63_817, _63_819) -> begin
 (
 
-let _63_652 = (FStar_Syntax_Util.arrow_formals t)
-in (match (_63_652) with
-| (formals, _63_651) -> begin
+let _63_825 = (FStar_Syntax_Util.arrow_formals t)
+in (match (_63_825) with
+| (formals, _63_824) -> begin
 (
 
 let is_rec = (is_rec tags)
 in (
 
-let fields = (FStar_All.pipe_right formals (FStar_List.collect (fun _63_656 -> (match (_63_656) with
+let fields = (FStar_All.pipe_right formals (FStar_List.collect (fun _63_829 -> (match (_63_829) with
 | (x, q) -> begin
 if ((FStar_Syntax_Syntax.is_null_bv x) || (is_rec && (FStar_Syntax_Syntax.is_implicit q))) then begin
 []
 end else begin
-(let _158_411 = (let _158_410 = (let _158_409 = if is_rec then begin
+(let _158_674 = (let _158_673 = (let _158_672 = if is_rec then begin
 (FStar_Syntax_Util.unmangle_field_name x.FStar_Syntax_Syntax.ppname)
 end else begin
 x.FStar_Syntax_Syntax.ppname
 end
-in (FStar_Syntax_Util.mk_field_projector_name_from_ident constrname _158_409))
-in ((_158_410), (x.FStar_Syntax_Syntax.sort)))
-in (_158_411)::[])
+in (FStar_Syntax_Util.mk_field_projector_name_from_ident constrname _158_672))
+in ((_158_673), (x.FStar_Syntax_Syntax.sort)))
+in (_158_674)::[])
 end
 end))))
 in (
 
 let record = {typename = typename; constrname = constrname; parms = parms; fields = fields; is_record = is_rec}
-in (insert_record_cache record))))
+in (
+
+let _63_832 = (let _158_676 = (let _158_675 = (FStar_ST.read new_globs)
+in (Record_or_dc (record))::_158_675)
+in (FStar_ST.op_Colon_Equals new_globs _158_676))
+in (match (()) with
+| () -> begin
+(insert_record_cache record)
+end)))))
 end))
 end
-| _63_660 -> begin
+| _63_834 -> begin
 ()
 end)
 end
-| _63_662 -> begin
+| _63_836 -> begin
 ()
 end))))))
 end
-| _63_664 -> begin
+| _63_838 -> begin
 ()
 end))
 
 
-let try_lookup_record_or_dc_by_field_name : env  ->  FStar_Ident.lident  ->  (record_or_dc * FStar_Ident.lident) Prims.option = (fun env fieldname -> (
+let try_lookup_record_or_dc_by_field_name : env  ->  FStar_Ident.lident  ->  (record_or_dc * FStar_Syntax_Syntax.fieldname) Prims.option = (fun env fieldname -> (
 
 let needs_constrname = (not ((FStar_Syntax_Util.field_projector_contains_constructor fieldname.FStar_Ident.ident.FStar_Ident.idText)))
 in (
 
 let find_in_cache = (fun fieldname -> (
 
-let _63_672 = ((fieldname.FStar_Ident.ns), (fieldname.FStar_Ident.ident))
-in (match (_63_672) with
+let _63_846 = ((fieldname.FStar_Ident.ns), (fieldname.FStar_Ident.ident))
+in (match (_63_846) with
 | (ns, id) -> begin
-(let _158_421 = (peek_record_cache ())
-in (FStar_Util.find_map _158_421 (fun record -> (
-
-let constrname = record.constrname.FStar_Ident.ident
-in (
-
-let fname = if needs_constrname then begin
-(let _158_419 = (FStar_Ident.lid_of_ids (FStar_List.append ns ((constrname)::[])))
-in (FStar_Syntax_Util.mk_field_projector_name_from_ident _158_419 id))
-end else begin
-fieldname
-end
-in (FStar_Util.find_map record.fields (fun _63_679 -> (match (_63_679) with
-| (f, _63_678) -> begin
-if (FStar_Ident.lid_equals fname f) then begin
-Some (((record), (fname)))
-end else begin
-None
-end
-end))))))))
+(let _158_687 = (peek_record_cache ())
+in (FStar_Util.find_map _158_687 (fun record -> (let _158_686 = (find_in_record ns id record (fun r -> Cont_ok (r)))
+in (option_of_cont (fun _63_849 -> None) _158_686)))))
 end)))
-in (resolve_in_open_namespaces env fieldname find_in_cache))))
+in (resolve_in_open_namespaces'' env fieldname (fun _63_859 -> Cont_ignore) (fun _63_857 -> Cont_ignore) (fun r -> Cont_ok (r)) (fun k fn -> (let _158_693 = (find_in_cache fn)
+in (cont_of_option k _158_693))) (fun k _63_852 -> k)))))
 
 
 let try_lookup_record_by_field_name : env  ->  FStar_Ident.lident  ->  (record_or_dc * FStar_Ident.lident) Prims.option = (fun env fieldname -> (match ((try_lookup_record_or_dc_by_field_name env fieldname)) with
 | Some (r, f) when r.is_record -> begin
 Some (((r), (f)))
 end
-| _63_687 -> begin
+| _63_868 -> begin
 None
 end))
 
@@ -780,7 +1104,7 @@ let try_lookup_projector_by_field_name : env  ->  FStar_Ident.lident  ->  (FStar
 | Some (r, f) -> begin
 Some (((f), (r.is_record)))
 end
-| _63_695 -> begin
+| _63_876 -> begin
 None
 end))
 
@@ -789,18 +1113,18 @@ let qualify_field_to_record : env  ->  record_or_dc  ->  FStar_Ident.lident  -> 
 
 let qualify = (fun fieldname -> (
 
-let _63_703 = ((fieldname.FStar_Ident.ns), (fieldname.FStar_Ident.ident))
-in (match (_63_703) with
+let _63_884 = ((fieldname.FStar_Ident.ns), (fieldname.FStar_Ident.ident))
+in (match (_63_884) with
 | (ns, fieldname) -> begin
 (
 
 let constrname = recd.constrname.FStar_Ident.ident
 in (
 
-let fname = (let _158_438 = (FStar_Ident.lid_of_ids (FStar_List.append ns ((constrname)::[])))
-in (FStar_Syntax_Util.mk_field_projector_name_from_ident _158_438 fieldname))
-in (FStar_Util.find_map recd.fields (fun _63_709 -> (match (_63_709) with
-| (f, _63_708) -> begin
+let fname = (let _158_712 = (FStar_Ident.lid_of_ids (FStar_List.append ns ((constrname)::[])))
+in (FStar_Syntax_Util.mk_field_projector_name_from_ident _158_712 fieldname))
+in (FStar_Util.find_map recd.fields (fun _63_890 -> (match (_63_890) with
+| (f, _63_889) -> begin
 if (FStar_Ident.lid_equals fname f) then begin
 Some (fname)
 end else begin
@@ -808,31 +1132,35 @@ None
 end
 end)))))
 end)))
-in (resolve_in_open_namespaces env f qualify)))
+in (resolve_in_open_namespaces'' env f (fun _63_899 -> Cont_ignore) (fun _63_897 -> Cont_ignore) (fun r -> Cont_ok ((Prims.snd r))) (fun k fn -> (let _158_719 = (qualify fn)
+in (cont_of_option k _158_719))) (fun k _63_892 -> k))))
 
 
 let unique : Prims.bool  ->  Prims.bool  ->  env  ->  FStar_Ident.lident  ->  Prims.bool = (fun any_val exclude_if env lid -> (
 
 let this_env = (
 
-let _63_714 = env
-in {curmodule = _63_714.curmodule; curmonad = _63_714.curmonad; modules = _63_714.modules; open_namespaces = []; modul_abbrevs = _63_714.modul_abbrevs; sigaccum = _63_714.sigaccum; localbindings = _63_714.localbindings; recbindings = _63_714.recbindings; sigmap = _63_714.sigmap; default_result_effect = _63_714.default_result_effect; iface = _63_714.iface; admitted_iface = _63_714.admitted_iface; expect_typ = _63_714.expect_typ})
+let _63_905 = env
+in {curmodule = _63_905.curmodule; curmonad = _63_905.curmonad; modules = _63_905.modules; scope_mods = []; sigaccum = _63_905.sigaccum; sigmap = _63_905.sigmap; default_result_effect = _63_905.default_result_effect; iface = _63_905.iface; admitted_iface = _63_905.admitted_iface; expect_typ = _63_905.expect_typ})
 in (match ((try_lookup_lid' any_val exclude_if env lid)) with
 | None -> begin
 true
 end
-| Some (_63_719) -> begin
+| Some (_63_910) -> begin
 false
 end)))
+
+
+let push_scope_mod : env  ->  scope_mod  ->  env = (fun env scope_mod -> (
+
+let _63_914 = env
+in {curmodule = _63_914.curmodule; curmonad = _63_914.curmonad; modules = _63_914.modules; scope_mods = (scope_mod)::env.scope_mods; sigaccum = _63_914.sigaccum; sigmap = _63_914.sigmap; default_result_effect = _63_914.default_result_effect; iface = _63_914.iface; admitted_iface = _63_914.admitted_iface; expect_typ = _63_914.expect_typ}))
 
 
 let push_bv' : env  ->  FStar_Ident.ident  ->  Prims.bool  ->  (env * FStar_Syntax_Syntax.bv) = (fun env x is_mutable -> (
 
 let bv = (FStar_Syntax_Syntax.gen_bv x.FStar_Ident.idText (Some (x.FStar_Ident.idRange)) FStar_Syntax_Syntax.tun)
-in (((
-
-let _63_725 = env
-in {curmodule = _63_725.curmodule; curmonad = _63_725.curmonad; modules = _63_725.modules; open_namespaces = _63_725.open_namespaces; modul_abbrevs = _63_725.modul_abbrevs; sigaccum = _63_725.sigaccum; localbindings = (((x), (bv), (is_mutable)))::env.localbindings; recbindings = _63_725.recbindings; sigmap = _63_725.sigmap; default_result_effect = _63_725.default_result_effect; iface = _63_725.iface; admitted_iface = _63_725.admitted_iface; expect_typ = _63_725.expect_typ})), (bv))))
+in (((push_scope_mod env (Local_binding (((x), (bv), (is_mutable)))))), (bv))))
 
 
 let push_bv_mutable : env  ->  FStar_Ident.ident  ->  (env * FStar_Syntax_Syntax.bv) = (fun env x -> (push_bv' env x true))
@@ -845,10 +1173,7 @@ let push_top_level_rec_binding : env  ->  FStar_Ident.ident  ->  FStar_Syntax_Sy
 
 let l = (qualify env x)
 in if (unique false true env l) then begin
-(
-
-let _63_735 = env
-in {curmodule = _63_735.curmodule; curmonad = _63_735.curmonad; modules = _63_735.modules; open_namespaces = _63_735.open_namespaces; modul_abbrevs = _63_735.modul_abbrevs; sigaccum = _63_735.sigaccum; localbindings = _63_735.localbindings; recbindings = (((x), (l), (dd)))::env.recbindings; sigmap = _63_735.sigmap; default_result_effect = _63_735.default_result_effect; iface = _63_735.iface; admitted_iface = _63_735.admitted_iface; expect_typ = _63_735.expect_typ})
+(push_scope_mod env (Rec_binding (((x), (l), (dd)))))
 end else begin
 (Prims.raise (FStar_Syntax_Syntax.Error ((((Prims.strcat "Duplicate top-level names " l.FStar_Ident.str)), ((FStar_Ident.range_of_lid l))))))
 end))
@@ -862,9 +1187,9 @@ let sopt = (FStar_Util.smap_try_find (sigmap env) l.FStar_Ident.str)
 in (
 
 let r = (match (sopt) with
-| Some (se, _63_744) -> begin
-(match ((let _158_474 = (FStar_Syntax_Util.lids_of_sigelt se)
-in (FStar_Util.find_opt (FStar_Ident.lid_equals l) _158_474))) with
+| Some (se, _63_935) -> begin
+(match ((let _158_760 = (FStar_Syntax_Util.lids_of_sigelt se)
+in (FStar_Util.find_opt (FStar_Ident.lid_equals l) _158_760))) with
 | Some (l) -> begin
 (FStar_All.pipe_left FStar_Range.string_of_range (FStar_Ident.range_of_lid l))
 end
@@ -875,25 +1200,28 @@ end
 | None -> begin
 "<unknown>"
 end)
-in (let _158_477 = (let _158_476 = (let _158_475 = (FStar_Util.format2 "Duplicate top-level names [%s]; previously declared at %s" (FStar_Ident.text_of_lid l) r)
-in ((_158_475), ((FStar_Ident.range_of_lid l))))
-in FStar_Syntax_Syntax.Error (_158_476))
-in (Prims.raise _158_477)))))
+in (let _158_763 = (let _158_762 = (let _158_761 = (FStar_Util.format2 "Duplicate top-level names [%s]; previously declared at %s" (FStar_Ident.text_of_lid l) r)
+in ((_158_761), ((FStar_Ident.range_of_lid l))))
+in FStar_Syntax_Syntax.Error (_158_762))
+in (Prims.raise _158_763)))))
+in (
+
+let globals = (FStar_ST.alloc env.scope_mods)
 in (
 
 let env = (
 
-let _63_762 = (match (s) with
-| FStar_Syntax_Syntax.Sig_let (_63_753) -> begin
+let _63_954 = (match (s) with
+| FStar_Syntax_Syntax.Sig_let (_63_945) -> begin
 ((false), (true))
 end
-| FStar_Syntax_Syntax.Sig_bundle (_63_756) -> begin
+| FStar_Syntax_Syntax.Sig_bundle (_63_948) -> begin
 ((true), (true))
 end
-| _63_759 -> begin
+| _63_951 -> begin
 ((false), (false))
 end)
-in (match (_63_762) with
+in (match (_63_954) with
 | (any_val, exclude_if) -> begin
 (
 
@@ -906,11 +1234,11 @@ end))) with
 | None -> begin
 (
 
-let _63_766 = (extract_record env s)
+let _63_958 = (extract_record env globals s)
 in (
 
-let _63_768 = env
-in {curmodule = _63_768.curmodule; curmonad = _63_768.curmonad; modules = _63_768.modules; open_namespaces = _63_768.open_namespaces; modul_abbrevs = _63_768.modul_abbrevs; sigaccum = (s)::env.sigaccum; localbindings = _63_768.localbindings; recbindings = _63_768.recbindings; sigmap = _63_768.sigmap; default_result_effect = _63_768.default_result_effect; iface = _63_768.iface; admitted_iface = _63_768.admitted_iface; expect_typ = _63_768.expect_typ}))
+let _63_960 = env
+in {curmodule = _63_960.curmodule; curmonad = _63_960.curmonad; modules = _63_960.modules; scope_mods = _63_960.scope_mods; sigaccum = (s)::env.sigaccum; sigmap = _63_960.sigmap; default_result_effect = _63_960.default_result_effect; iface = _63_960.iface; admitted_iface = _63_960.admitted_iface; expect_typ = _63_960.expect_typ}))
 end
 | Some (l) -> begin
 (err l)
@@ -918,76 +1246,90 @@ end))
 end))
 in (
 
-let _63_787 = (match (s) with
-| FStar_Syntax_Syntax.Sig_bundle (ses, _63_775, _63_777, _63_779) -> begin
-(let _158_481 = (FStar_List.map (fun se -> (let _158_480 = (FStar_Syntax_Util.lids_of_sigelt se)
-in ((_158_480), (se)))) ses)
-in ((env), (_158_481)))
+let env = (
+
+let _63_965 = env
+in (let _158_765 = (FStar_ST.read globals)
+in {curmodule = _63_965.curmodule; curmonad = _63_965.curmonad; modules = _63_965.modules; scope_mods = _158_765; sigaccum = _63_965.sigaccum; sigmap = _63_965.sigmap; default_result_effect = _63_965.default_result_effect; iface = _63_965.iface; admitted_iface = _63_965.admitted_iface; expect_typ = _63_965.expect_typ}))
+in (
+
+let _63_982 = (match (s) with
+| FStar_Syntax_Syntax.Sig_bundle (ses, _63_970, _63_972, _63_974) -> begin
+(let _158_768 = (FStar_List.map (fun se -> (let _158_767 = (FStar_Syntax_Util.lids_of_sigelt se)
+in ((_158_767), (se)))) ses)
+in ((env), (_158_768)))
 end
-| _63_784 -> begin
-(let _158_484 = (let _158_483 = (let _158_482 = (FStar_Syntax_Util.lids_of_sigelt s)
-in ((_158_482), (s)))
-in (_158_483)::[])
-in ((env), (_158_484)))
+| _63_979 -> begin
+(let _158_771 = (let _158_770 = (let _158_769 = (FStar_Syntax_Util.lids_of_sigelt s)
+in ((_158_769), (s)))
+in (_158_770)::[])
+in ((env), (_158_771)))
 end)
-in (match (_63_787) with
+in (match (_63_982) with
 | (env, lss) -> begin
 (
 
-let _63_792 = (FStar_All.pipe_right lss (FStar_List.iter (fun _63_790 -> (match (_63_790) with
+let _63_988 = (FStar_All.pipe_right lss (FStar_List.iter (fun _63_985 -> (match (_63_985) with
 | (lids, se) -> begin
-(FStar_All.pipe_right lids (FStar_List.iter (fun lid -> (FStar_Util.smap_add (sigmap env) lid.FStar_Ident.str ((se), ((env.iface && (not (env.admitted_iface)))))))))
-end))))
-in env)
+(FStar_All.pipe_right lids (FStar_List.iter (fun lid -> (
+
+let _63_987 = (let _158_775 = (let _158_774 = (FStar_ST.read globals)
+in (Top_level_def (lid.FStar_Ident.ident))::_158_774)
+in (FStar_ST.op_Colon_Equals globals _158_775))
+in (match (()) with
+| () -> begin
+(FStar_Util.smap_add (sigmap env) lid.FStar_Ident.str ((se), ((env.iface && (not (env.admitted_iface))))))
 end)))))
+end))))
+in (
+
+let env = (
+
+let _63_990 = env
+in (let _158_776 = (FStar_ST.read globals)
+in {curmodule = _63_990.curmodule; curmonad = _63_990.curmonad; modules = _63_990.modules; scope_mods = _158_776; sigaccum = _63_990.sigaccum; sigmap = _63_990.sigmap; default_result_effect = _63_990.default_result_effect; iface = _63_990.iface; admitted_iface = _63_990.admitted_iface; expect_typ = _63_990.expect_typ}))
+in env))
+end)))))))
 
 
 let push_namespace : env  ->  FStar_Ident.lident  ->  env = (fun env ns -> (
 
-let modules = env.modules
-in if (FStar_All.pipe_right modules (FStar_Util.for_some (fun _63_800 -> (match (_63_800) with
-| (m, _63_799) -> begin
-(FStar_Util.starts_with (FStar_Ident.text_of_lid m) (FStar_Ident.text_of_lid ns))
-end)))) then begin
+let _63_1005 = (match ((resolve_module_name env ns)) with
+| None -> begin
 (
 
-let _63_801 = env
-in {curmodule = _63_801.curmodule; curmonad = _63_801.curmonad; modules = _63_801.modules; open_namespaces = (ns)::env.open_namespaces; modul_abbrevs = _63_801.modul_abbrevs; sigaccum = _63_801.sigaccum; localbindings = _63_801.localbindings; recbindings = _63_801.recbindings; sigmap = _63_801.sigmap; default_result_effect = _63_801.default_result_effect; iface = _63_801.iface; admitted_iface = _63_801.admitted_iface; expect_typ = _63_801.expect_typ})
+let modules = env.modules
+in if (FStar_All.pipe_right modules (FStar_Util.for_some (fun _63_1000 -> (match (_63_1000) with
+| (m, _63_999) -> begin
+(FStar_Util.starts_with (Prims.strcat (FStar_Ident.text_of_lid m) ".") (Prims.strcat (FStar_Ident.text_of_lid ns) "."))
+end)))) then begin
+((ns), (Open_namespace))
 end else begin
-(let _158_494 = (let _158_493 = (let _158_492 = (FStar_Util.format1 "Namespace %s cannot be found" (FStar_Ident.text_of_lid ns))
-in ((_158_492), ((FStar_Ident.range_of_lid ns))))
-in FStar_Syntax_Syntax.Error (_158_493))
-in (Prims.raise _158_494))
+(let _158_784 = (let _158_783 = (let _158_782 = (FStar_Util.format1 "Namespace %s cannot be found" (FStar_Ident.text_of_lid ns))
+in ((_158_782), ((FStar_Ident.range_of_lid ns))))
+in FStar_Syntax_Syntax.Error (_158_783))
+in (Prims.raise _158_784))
+end)
+end
+| Some (ns') -> begin
+((ns'), (Open_module))
+end)
+in (match (_63_1005) with
+| (ns', kd) -> begin
+(push_scope_mod env (Open_module_or_namespace (((ns'), (kd)))))
+end)))
+
+
+let push_module_abbrev : env  ->  FStar_Ident.ident  ->  FStar_Ident.lident  ->  env = (fun env x l -> (match ((resolve_module_name env l)) with
+| None -> begin
+(let _158_793 = (let _158_792 = (let _158_791 = (FStar_Util.format1 "Module %s cannot be found" (FStar_Ident.text_of_lid l))
+in ((_158_791), ((FStar_Ident.range_of_lid l))))
+in FStar_Syntax_Syntax.Error (_158_792))
+in (Prims.raise _158_793))
+end
+| Some (modul) -> begin
+(push_scope_mod env (Module_abbrev (((x), (modul)))))
 end))
-
-
-let push_module_abbrev : env  ->  FStar_Ident.ident  ->  FStar_Ident.lident  ->  env = (fun env x l -> if (FStar_All.pipe_right env.modul_abbrevs (FStar_Util.for_some (fun _63_809 -> (match (_63_809) with
-| (y, _63_808) -> begin
-(x.FStar_Ident.idText = y.FStar_Ident.idText)
-end)))) then begin
-(let _158_504 = (let _158_503 = (let _158_502 = (FStar_Util.format1 "Module %s is already defined" x.FStar_Ident.idText)
-in ((_158_502), (x.FStar_Ident.idRange)))
-in FStar_Syntax_Syntax.Error (_158_503))
-in (Prims.raise _158_504))
-end else begin
-(
-
-let modules = env.modules
-in if (FStar_All.pipe_right modules (FStar_Util.for_some (fun _63_814 -> (match (_63_814) with
-| (m, _63_813) -> begin
-(FStar_Ident.lid_equals m l)
-end)))) then begin
-(
-
-let _63_815 = env
-in {curmodule = _63_815.curmodule; curmonad = _63_815.curmonad; modules = _63_815.modules; open_namespaces = _63_815.open_namespaces; modul_abbrevs = (((x), (l)))::env.modul_abbrevs; sigaccum = _63_815.sigaccum; localbindings = _63_815.localbindings; recbindings = _63_815.recbindings; sigmap = _63_815.sigmap; default_result_effect = _63_815.default_result_effect; iface = _63_815.iface; admitted_iface = _63_815.admitted_iface; expect_typ = _63_815.expect_typ})
-end else begin
-(let _158_508 = (let _158_507 = (let _158_506 = (FStar_Util.format1 "Module %s cannot be found" (FStar_Ident.text_of_lid l))
-in ((_158_506), ((FStar_Ident.range_of_lid l))))
-in FStar_Syntax_Syntax.Error (_158_507))
-in (Prims.raise _158_508))
-end)
-end)
 
 
 let check_admits : env  ->  Prims.unit = (fun env -> (FStar_All.pipe_right env.sigaccum (FStar_List.iter (fun se -> (match (se) with
@@ -996,62 +1338,62 @@ let check_admits : env  ->  Prims.unit = (fun env -> (FStar_All.pipe_right env.s
 | None -> begin
 (
 
-let _63_827 = (let _158_514 = (let _158_513 = (FStar_Range.string_of_range (FStar_Ident.range_of_lid l))
-in (let _158_512 = (FStar_Syntax_Print.lid_to_string l)
-in (FStar_Util.format2 "%s: Warning: Admitting %s without a definition\n" _158_513 _158_512)))
-in (FStar_Util.print_string _158_514))
+let _63_1022 = (let _158_799 = (let _158_798 = (FStar_Range.string_of_range (FStar_Ident.range_of_lid l))
+in (let _158_797 = (FStar_Syntax_Print.lid_to_string l)
+in (FStar_Util.format2 "%s: Warning: Admitting %s without a definition\n" _158_798 _158_797)))
+in (FStar_Util.print_string _158_799))
 in (FStar_Util.smap_add (sigmap env) l.FStar_Ident.str ((FStar_Syntax_Syntax.Sig_declare_typ (((l), (u), (t), ((FStar_Syntax_Syntax.Assumption)::quals), (r)))), (false))))
 end
-| Some (_63_830) -> begin
+| Some (_63_1025) -> begin
 ()
 end)
 end
-| _63_833 -> begin
+| _63_1028 -> begin
 ()
 end)))))
 
 
 let finish : env  ->  FStar_Syntax_Syntax.modul  ->  env = (fun env modul -> (
 
-let _63_893 = (FStar_All.pipe_right modul.FStar_Syntax_Syntax.declarations (FStar_List.iter (fun _63_13 -> (match (_63_13) with
-| FStar_Syntax_Syntax.Sig_bundle (ses, quals, _63_840, _63_842) -> begin
+let _63_1088 = (FStar_All.pipe_right modul.FStar_Syntax_Syntax.declarations (FStar_List.iter (fun _63_25 -> (match (_63_25) with
+| FStar_Syntax_Syntax.Sig_bundle (ses, quals, _63_1035, _63_1037) -> begin
 if ((FStar_List.contains FStar_Syntax_Syntax.Private quals) || (FStar_List.contains FStar_Syntax_Syntax.Abstract quals)) then begin
-(FStar_All.pipe_right ses (FStar_List.iter (fun _63_12 -> (match (_63_12) with
-| FStar_Syntax_Syntax.Sig_datacon (lid, _63_848, _63_850, _63_852, _63_854, _63_856, _63_858, _63_860) -> begin
+(FStar_All.pipe_right ses (FStar_List.iter (fun _63_24 -> (match (_63_24) with
+| FStar_Syntax_Syntax.Sig_datacon (lid, _63_1043, _63_1045, _63_1047, _63_1049, _63_1051, _63_1053, _63_1055) -> begin
 (FStar_Util.smap_remove (sigmap env) lid.FStar_Ident.str)
 end
-| _63_864 -> begin
+| _63_1059 -> begin
 ()
 end))))
 end else begin
 ()
 end
 end
-| FStar_Syntax_Syntax.Sig_declare_typ (lid, _63_867, _63_869, quals, _63_872) -> begin
+| FStar_Syntax_Syntax.Sig_declare_typ (lid, _63_1062, _63_1064, quals, _63_1067) -> begin
 if (FStar_List.contains FStar_Syntax_Syntax.Private quals) then begin
 (FStar_Util.smap_remove (sigmap env) lid.FStar_Ident.str)
 end else begin
 ()
 end
 end
-| FStar_Syntax_Syntax.Sig_let ((_63_876, lbs), r, _63_881, quals) -> begin
+| FStar_Syntax_Syntax.Sig_let ((_63_1071, lbs), r, _63_1076, quals) -> begin
 (
 
-let _63_886 = if ((FStar_List.contains FStar_Syntax_Syntax.Private quals) || (FStar_List.contains FStar_Syntax_Syntax.Abstract quals)) then begin
-(FStar_All.pipe_right lbs (FStar_List.iter (fun lb -> (let _158_525 = (let _158_524 = (let _158_523 = (let _158_522 = (FStar_Util.right lb.FStar_Syntax_Syntax.lbname)
-in _158_522.FStar_Syntax_Syntax.fv_name)
-in _158_523.FStar_Syntax_Syntax.v)
-in _158_524.FStar_Ident.str)
-in (FStar_Util.smap_remove (sigmap env) _158_525)))))
+let _63_1081 = if ((FStar_List.contains FStar_Syntax_Syntax.Private quals) || (FStar_List.contains FStar_Syntax_Syntax.Abstract quals)) then begin
+(FStar_All.pipe_right lbs (FStar_List.iter (fun lb -> (let _158_810 = (let _158_809 = (let _158_808 = (let _158_807 = (FStar_Util.right lb.FStar_Syntax_Syntax.lbname)
+in _158_807.FStar_Syntax_Syntax.fv_name)
+in _158_808.FStar_Syntax_Syntax.v)
+in _158_809.FStar_Ident.str)
+in (FStar_Util.smap_remove (sigmap env) _158_810)))))
 end else begin
 ()
 end
 in if ((FStar_List.contains FStar_Syntax_Syntax.Abstract quals) && (not ((FStar_List.contains FStar_Syntax_Syntax.Private quals)))) then begin
 (FStar_All.pipe_right lbs (FStar_List.iter (fun lb -> (
 
-let lid = (let _158_528 = (let _158_527 = (FStar_Util.right lb.FStar_Syntax_Syntax.lbname)
-in _158_527.FStar_Syntax_Syntax.fv_name)
-in _158_528.FStar_Syntax_Syntax.v)
+let lid = (let _158_813 = (let _158_812 = (FStar_Util.right lb.FStar_Syntax_Syntax.lbname)
+in _158_812.FStar_Syntax_Syntax.fv_name)
+in _158_813.FStar_Syntax_Syntax.v)
 in (
 
 let decl = FStar_Syntax_Syntax.Sig_declare_typ (((lid), (lb.FStar_Syntax_Syntax.lbunivs), (lb.FStar_Syntax_Syntax.lbtyp), ((FStar_Syntax_Syntax.Assumption)::quals), (r)))
@@ -1060,13 +1402,13 @@ end else begin
 ()
 end)
 end
-| _63_892 -> begin
+| _63_1087 -> begin
 ()
 end))))
 in (
 
-let _63_895 = env
-in {curmodule = None; curmonad = _63_895.curmonad; modules = (((modul.FStar_Syntax_Syntax.name), (modul)))::env.modules; open_namespaces = []; modul_abbrevs = []; sigaccum = []; localbindings = []; recbindings = []; sigmap = _63_895.sigmap; default_result_effect = _63_895.default_result_effect; iface = _63_895.iface; admitted_iface = _63_895.admitted_iface; expect_typ = _63_895.expect_typ})))
+let _63_1090 = env
+in {curmodule = None; curmonad = _63_1090.curmonad; modules = (((modul.FStar_Syntax_Syntax.name), (modul)))::env.modules; scope_mods = []; sigaccum = []; sigmap = _63_1090.sigmap; default_result_effect = _63_1090.default_result_effect; iface = _63_1090.iface; admitted_iface = _63_1090.admitted_iface; expect_typ = _63_1090.expect_typ})))
 
 
 type env_stack_ops =
@@ -1083,45 +1425,45 @@ in (
 
 let push = (fun env -> (
 
-let _63_906 = (push_record_cache ())
+let _63_1101 = (push_record_cache ())
 in (
 
-let _63_908 = (let _158_578 = (let _158_577 = (FStar_ST.read stack)
-in (env)::_158_577)
-in (FStar_ST.op_Colon_Equals stack _158_578))
+let _63_1103 = (let _158_863 = (let _158_862 = (FStar_ST.read stack)
+in (env)::_158_862)
+in (FStar_ST.op_Colon_Equals stack _158_863))
 in (
 
-let _63_910 = env
-in (let _158_579 = (FStar_Util.smap_copy (sigmap env))
-in {curmodule = _63_910.curmodule; curmonad = _63_910.curmonad; modules = _63_910.modules; open_namespaces = _63_910.open_namespaces; modul_abbrevs = _63_910.modul_abbrevs; sigaccum = _63_910.sigaccum; localbindings = _63_910.localbindings; recbindings = _63_910.recbindings; sigmap = _158_579; default_result_effect = _63_910.default_result_effect; iface = _63_910.iface; admitted_iface = _63_910.admitted_iface; expect_typ = _63_910.expect_typ})))))
+let _63_1105 = env
+in (let _158_864 = (FStar_Util.smap_copy (sigmap env))
+in {curmodule = _63_1105.curmodule; curmonad = _63_1105.curmonad; modules = _63_1105.modules; scope_mods = _63_1105.scope_mods; sigaccum = _63_1105.sigaccum; sigmap = _158_864; default_result_effect = _63_1105.default_result_effect; iface = _63_1105.iface; admitted_iface = _63_1105.admitted_iface; expect_typ = _63_1105.expect_typ})))))
 in (
 
 let pop = (fun env -> (match ((FStar_ST.read stack)) with
 | (env)::tl -> begin
 (
 
-let _63_917 = (pop_record_cache ())
+let _63_1112 = (pop_record_cache ())
 in (
 
-let _63_919 = (FStar_ST.op_Colon_Equals stack tl)
+let _63_1114 = (FStar_ST.op_Colon_Equals stack tl)
 in env))
 end
-| _63_922 -> begin
+| _63_1117 -> begin
 (FStar_All.failwith "Impossible: Too many pops")
 end))
 in (
 
 let commit_mark = (fun env -> (
 
-let _63_925 = (commit_record_cache ())
+let _63_1120 = (commit_record_cache ())
 in (match ((FStar_ST.read stack)) with
-| (_63_929)::tl -> begin
+| (_63_1124)::tl -> begin
 (
 
-let _63_931 = (FStar_ST.op_Colon_Equals stack tl)
+let _63_1126 = (FStar_ST.op_Colon_Equals stack tl)
 in env)
 end
-| _63_934 -> begin
+| _63_1129 -> begin
 (FStar_All.failwith "Impossible: Too many pops")
 end)))
 in {push = push; mark = push; reset_mark = pop; commit_mark = commit_mark; pop = pop}))))
@@ -1145,10 +1487,10 @@ let pop : env  ->  env = (fun env -> (stack_ops.pop env))
 let export_interface : FStar_Ident.lident  ->  env  ->  env = (fun m env -> (
 
 let sigelt_in_m = (fun se -> (match ((FStar_Syntax_Util.lids_of_sigelt se)) with
-| (l)::_63_945 -> begin
+| (l)::_63_1140 -> begin
 (l.FStar_Ident.nsstr = m.FStar_Ident.str)
 end
-| _63_949 -> begin
+| _63_1144 -> begin
 false
 end))
 in (
@@ -1165,23 +1507,23 @@ in (
 let sm' = (sigmap env)
 in (
 
-let _63_973 = (FStar_All.pipe_right keys (FStar_List.iter (fun k -> (match ((FStar_Util.smap_try_find sm' k)) with
+let _63_1168 = (FStar_All.pipe_right keys (FStar_List.iter (fun k -> (match ((FStar_Util.smap_try_find sm' k)) with
 | Some (se, true) when (sigelt_in_m se) -> begin
 (
 
-let _63_959 = (FStar_Util.smap_remove sm' k)
+let _63_1154 = (FStar_Util.smap_remove sm' k)
 in (
 
 let se = (match (se) with
 | FStar_Syntax_Syntax.Sig_declare_typ (l, u, t, q, r) -> begin
 FStar_Syntax_Syntax.Sig_declare_typ (((l), (u), (t), ((FStar_Syntax_Syntax.Assumption)::q), (r)))
 end
-| _63_969 -> begin
+| _63_1164 -> begin
 se
 end)
 in (FStar_Util.smap_add sm' k ((se), (false)))))
 end
-| _63_972 -> begin
+| _63_1167 -> begin
 ()
 end))))
 in env)))))))
@@ -1189,7 +1531,7 @@ in env)))))))
 
 let finish_module_or_interface : env  ->  FStar_Syntax_Syntax.modul  ->  env = (fun env modul -> (
 
-let _63_977 = if (not (modul.FStar_Syntax_Syntax.is_interface)) then begin
+let _63_1172 = if (not (modul.FStar_Syntax_Syntax.is_interface)) then begin
 (check_admits env)
 end else begin
 ()
@@ -1222,34 +1564,35 @@ open_ns
 end
 in (
 
-let _63_988 = env
-in {curmodule = Some (mname); curmonad = _63_988.curmonad; modules = _63_988.modules; open_namespaces = open_ns; modul_abbrevs = _63_988.modul_abbrevs; sigaccum = _63_988.sigaccum; localbindings = _63_988.localbindings; recbindings = _63_988.recbindings; sigmap = env.sigmap; default_result_effect = if ((FStar_Ident.lid_equals mname FStar_Syntax_Const.all_lid) || (has_all_in_scope env)) then begin
+let _63_1183 = env
+in (let _158_901 = (FStar_List.map (fun lid -> Open_module_or_namespace (((lid), (Open_namespace)))) open_ns)
+in {curmodule = Some (mname); curmonad = _63_1183.curmonad; modules = _63_1183.modules; scope_mods = _158_901; sigaccum = _63_1183.sigaccum; sigmap = env.sigmap; default_result_effect = if ((FStar_Ident.lid_equals mname FStar_Syntax_Const.all_lid) || (has_all_in_scope env)) then begin
 FStar_Syntax_Const.effect_ML_lid
 end else begin
 FStar_Syntax_Const.effect_Tot_lid
-end; iface = intf; admitted_iface = admitted; expect_typ = _63_988.expect_typ}))))
-in (match ((FStar_All.pipe_right env.modules (FStar_Util.find_opt (fun _63_993 -> (match (_63_993) with
-| (l, _63_992) -> begin
+end; iface = intf; admitted_iface = admitted; expect_typ = _63_1183.expect_typ})))))
+in (match ((FStar_All.pipe_right env.modules (FStar_Util.find_opt (fun _63_1189 -> (match (_63_1189) with
+| (l, _63_1188) -> begin
 (FStar_Ident.lid_equals l mname)
 end))))) with
 | None -> begin
-(let _158_616 = (prep env)
-in ((_158_616), (false)))
+(let _158_903 = (prep env)
+in ((_158_903), (false)))
 end
-| Some (_63_996, m) -> begin
+| Some (_63_1192, m) -> begin
 (
 
-let _63_1000 = if ((not (m.FStar_Syntax_Syntax.is_interface)) || intf) then begin
-(let _158_619 = (let _158_618 = (let _158_617 = (FStar_Util.format1 "Duplicate module or interface name: %s" mname.FStar_Ident.str)
-in ((_158_617), ((FStar_Ident.range_of_lid mname))))
-in FStar_Syntax_Syntax.Error (_158_618))
-in (Prims.raise _158_619))
+let _63_1196 = if ((not (m.FStar_Syntax_Syntax.is_interface)) || intf) then begin
+(let _158_906 = (let _158_905 = (let _158_904 = (FStar_Util.format1 "Duplicate module or interface name: %s" mname.FStar_Ident.str)
+in ((_158_904), ((FStar_Ident.range_of_lid mname))))
+in FStar_Syntax_Syntax.Error (_158_905))
+in (Prims.raise _158_906))
 end else begin
 ()
 end
-in (let _158_621 = (let _158_620 = (push env)
-in (prep _158_620))
-in ((_158_621), (true))))
+in (let _158_908 = (let _158_907 = (push env)
+in (prep _158_907))
+in ((_158_908), (true))))
 end)))
 
 
@@ -1260,8 +1603,8 @@ end
 | None -> begin
 (
 
-let _63_1007 = env
-in {curmodule = _63_1007.curmodule; curmonad = Some (mname); modules = _63_1007.modules; open_namespaces = _63_1007.open_namespaces; modul_abbrevs = _63_1007.modul_abbrevs; sigaccum = _63_1007.sigaccum; localbindings = _63_1007.localbindings; recbindings = _63_1007.recbindings; sigmap = _63_1007.sigmap; default_result_effect = _63_1007.default_result_effect; iface = _63_1007.iface; admitted_iface = _63_1007.admitted_iface; expect_typ = _63_1007.expect_typ})
+let _63_1203 = env
+in {curmodule = _63_1203.curmodule; curmonad = Some (mname); modules = _63_1203.modules; scope_mods = _63_1203.scope_mods; sigaccum = _63_1203.sigaccum; sigmap = _63_1203.sigmap; default_result_effect = _63_1203.default_result_effect; iface = _63_1203.iface; admitted_iface = _63_1203.admitted_iface; expect_typ = _63_1203.expect_typ})
 end))
 
 
@@ -1269,34 +1612,40 @@ let fail_or = (fun env lookup lid -> (match ((lookup lid)) with
 | None -> begin
 (
 
-let opened_modules = (FStar_List.map (fun _63_1016 -> (match (_63_1016) with
-| (lid, _63_1015) -> begin
+let opened_modules = (FStar_List.map (fun _63_1212 -> (match (_63_1212) with
+| (lid, _63_1211) -> begin
 (FStar_Ident.text_of_lid lid)
 end)) env.modules)
-in (
-
-let module_of_the_lid = (let _158_633 = (FStar_Ident.path_of_ns lid.FStar_Ident.ns)
-in (FStar_Ident.text_of_path _158_633))
 in (
 
 let msg = (FStar_Util.format1 "Identifier not found: [%s]" (FStar_Ident.text_of_lid lid))
 in (
 
-let msg = (match (env.curmodule) with
-| Some (m) when (((FStar_Ident.text_of_lid m) = module_of_the_lid) || (module_of_the_lid = "")) -> begin
+let msg = if ((FStar_List.length lid.FStar_Ident.ns) = (Prims.parse_int "0")) then begin
 msg
+end else begin
+(
+
+let modul = (let _158_920 = (FStar_Ident.lid_of_ids lid.FStar_Ident.ns)
+in (FStar_Ident.set_lid_range _158_920 (FStar_Ident.range_of_lid lid)))
+in (match ((resolve_module_name env modul)) with
+| None -> begin
+(
+
+let opened_modules = (FStar_String.concat ", " opened_modules)
+in (FStar_Util.format3 "%s\nModule %s does not belong to the list of modules in scope, namely %s" msg modul.FStar_Ident.str opened_modules))
 end
-| _63_1023 when (FStar_List.existsb (fun m -> (m = module_of_the_lid)) opened_modules) -> begin
-msg
+| Some (modul') when (not ((FStar_List.existsb (fun m -> (m = modul'.FStar_Ident.str)) opened_modules))) -> begin
+(
+
+let opened_modules = (FStar_String.concat ", " opened_modules)
+in (FStar_Util.format4 "%s\nModule %s resolved into %s, which does not belong to the list of modules in scope, namely %s" msg modul.FStar_Ident.str modul'.FStar_Ident.str opened_modules))
 end
-| _63_1026 -> begin
-(let _158_638 = (let _158_637 = (let _158_636 = (let _158_635 = (FStar_Ident.path_of_ns lid.FStar_Ident.ns)
-in (FStar_Ident.text_of_path _158_635))
-in (FStar_Util.format3 "Hint: %s belongs to module %s, which does not belong to the list of modules in scope, namely %s" (FStar_Ident.text_of_lid lid) _158_636 (FStar_String.concat ", " opened_modules)))
-in (Prims.strcat "\n" _158_637))
-in (Prims.strcat msg _158_638))
-end)
-in (Prims.raise (FStar_Syntax_Syntax.Error (((msg), ((FStar_Ident.range_of_lid lid))))))))))
+| Some (modul') -> begin
+(FStar_Util.format4 "%s\nModule %s resolved into %s, definition %s not found" msg modul.FStar_Ident.str modul'.FStar_Ident.str lid.FStar_Ident.ident.FStar_Ident.idText)
+end))
+end
+in (Prims.raise (FStar_Syntax_Syntax.Error (((msg), ((FStar_Ident.range_of_lid lid)))))))))
 end
 | Some (r) -> begin
 r
